feat: map_unmap_ns_s1

container/coq/pointer/.CachedSpec/Layer7Spec.v
@@ -1,5 +1,15 @@
 Parameter test_PA : Z -> abs_PA_t.
 
+Parameter g_refcount_para : Ptr -> (RData -> Z).
+
+Definition s1tte_is_valid_spec_abs (v_0: abs_PTE_t) (v_1: Z) (st: RData) : (option (bool * RData)) :=
+  if ((v_1 =? (3)) && (((v_0.(meta_desc_type)) =? (3))))
+  then (Some (true, st))
+  else (
+    if ((v_1 <>? (3)) && (((v_0.(meta_desc_type)) =? (1))))
+    then (Some (true, st))
+    else (Some (false, st))).
+
 Definition s2tte_create_table_spec_abs (v_0: abs_PA_t) (v_1: Z) (st: RData) : (option (abs_PTE_t * RData)) :=
   (Some ((mkabs_PTE_t v_0 3 0), st)).
 
@@ -229,6 +239,96 @@ Definition rtt_create_internal_spec_abs (v_0: Ptr) (v_1_abs: abs_PA_t) (v_2: Z) 
           (Some ((pack_struct_return_code_para (make_return_code_para 8)), st_8))))))
   else (Some ((pack_struct_return_code_para (make_return_code_para 1)), st')).
 
-Definition rtt_create_internal_spec (v_0: Ptr) (v_1: Z) (v_2: Z) (v_3: Z) (v_4: Z) (st: RData) : (option (Z * RData)) :=
+Definition smc_granule_ns_to_any_spec_abs (v_0: Z) (v_1_abs: abs_PA_t) (st: RData) : (option (Z * RData)) :=
+  when st_1 == ((spinlock_acquire_spec (mkPtr "granules" (v_1_abs.(meta_granule_offset))) st));
+  if ((((((st_1.(share)).(globals)).(g_granules)) @ ((v_1_abs.(meta_granule_offset)) / (16))).(e_state_s_granule)) =? (0))
+  then (
+    rely (((((v_1_abs.(meta_granule_offset)) mod (16)) = (0)) /\ (((v_1_abs.(meta_granule_offset)) >= (0)))));
+    when st_6 == (
+        (granule_unlock_spec
+          (mkPtr "granules" (v_1_abs.(meta_granule_offset)))
+          (st_1.[share].[globals].[g_granules] :<
+            ((((st_1.(share)).(globals)).(g_granules)) #
+              ((v_1_abs.(meta_granule_offset)) / (16)) ==
+              ((((((st_1.(share)).(globals)).(g_granules)) @ ((v_1_abs.(meta_granule_offset)) / (16))).[e_ref] :<
+                ((((((st_1.(share)).(globals)).(g_granules)) @ ((v_1_abs.(meta_granule_offset)) / (16))).(e_ref)).[e_u_anon_3_0] :<
+                  ((g_mapped_addr_set_para ((((((st_1.(share)).(globals)).(g_granules)) @ ((v_1_abs.(meta_granule_offset)) / (16))).(e_ref)).(e_u_anon_3_0)) v_0) + (1)))).[e_state_s_granule] :<
+                6)))));
+    (Some (0, st_6)))
+  else (
+    when st_2 == ((spinlock_release_spec (mkPtr "granules" (v_1_abs.(meta_granule_offset))) st_1));
+    when st_3 == ((spinlock_acquire_spec (mkPtr "granules" (v_1_abs.(meta_granule_offset))) st_2));
+    if (((((((st_3.(share)).(globals)).(g_granules)) @ ((v_1_abs.(meta_granule_offset)) / (16))).(e_state_s_granule)) - (6)) =? (0))
+    then (
+      rely (((((v_1_abs.(meta_granule_offset)) mod (16)) = (0)) /\ (((v_1_abs.(meta_granule_offset)) >= (0)))));
+      rely (((((v_1_abs.(meta_granule_offset)) + (8)) mod (16)) = (8)));
+      when st_4 == (
+          (granule_unlock_spec
+            (mkPtr "granules" (v_1_abs.(meta_granule_offset)))
+            (st_3.[share].[globals].[g_granules] :<
+              ((((st_3.(share)).(globals)).(g_granules)) #
+                ((v_1_abs.(meta_granule_offset)) / (16)) ==
+                (((((st_3.(share)).(globals)).(g_granules)) @ ((v_1_abs.(meta_granule_offset)) / (16))).[e_ref] :<
+                  ((((((st_3.(share)).(globals)).(g_granules)) @ ((v_1_abs.(meta_granule_offset)) / (16))).(e_ref)).[e_u_anon_3_0] :<
+                    (((((((st_3.(share)).(globals)).(g_granules)) @ ((v_1_abs.(meta_granule_offset)) / (16))).(e_ref)).(e_u_anon_3_0)) + (1))))))));
+      (Some (0, st_4)))
+    else (
+      when st_4 == ((spinlock_release_spec (mkPtr "granules" (v_1_abs.(meta_granule_offset))) st_3));
+      (Some ((pack_struct_return_code_para (make_return_code_para 1)), st_4)))).
+
+Definition smc_granule_any_to_ns_spec_abs (v_0_abs: abs_PA_t) (st: RData) : (option (Z * RData)) :=
+  when st_1 == ((spinlock_acquire_spec (mkPtr "granules" (v_0_abs.(meta_granule_offset))) st));
+  if (((((((st_1.(share)).(globals)).(g_granules)) @ ((v_0_abs.(meta_granule_offset)) / (16))).(e_state_s_granule)) - (6)) =? (0))
+  then (
+    rely (((((v_0_abs.(meta_granule_offset)) mod (16)) = (0)) /\ (((v_0_abs.(meta_granule_offset)) >= (0)))));
+    if (
+      ((g_refcount_para
+        (mkPtr "granules" (v_0_abs.(meta_granule_offset)))
+        (st_1.[share].[globals].[g_granules] :<
+          ((((st_1.(share)).(globals)).(g_granules)) #
+            ((v_0_abs.(meta_granule_offset)) / (16)) ==
+            (((((st_1.(share)).(globals)).(g_granules)) @ ((v_0_abs.(meta_granule_offset)) / (16))).[e_ref] :<
+              ((((((st_1.(share)).(globals)).(g_granules)) @ ((v_0_abs.(meta_granule_offset)) / (16))).(e_ref)).[e_u_anon_3_0] :<
+                (((((((st_1.(share)).(globals)).(g_granules)) @ ((v_0_abs.(meta_granule_offset)) / (16))).(e_ref)).(e_u_anon_3_0)) + ((- 1)))))))) =?
+        (0)))
+    then (
+      when st_7 == (
+          (granule_unlock_spec
+            (mkPtr "granules" (v_0_abs.(meta_granule_offset)))
+            (st_1.[share].[globals].[g_granules] :<
+              ((((st_1.(share)).(globals)).(g_granules)) #
+                ((v_0_abs.(meta_granule_offset)) / (16)) ==
+                ((((((st_1.(share)).(globals)).(g_granules)) @ ((v_0_abs.(meta_granule_offset)) / (16))).[e_ref] :<
+                  ((((((st_1.(share)).(globals)).(g_granules)) @ ((v_0_abs.(meta_granule_offset)) / (16))).(e_ref)).[e_u_anon_3_0] :<
+                    (g_mapped_addr_set_para (((((((st_1.(share)).(globals)).(g_granules)) @ ((v_0_abs.(meta_granule_offset)) / (16))).(e_ref)).(e_u_anon_3_0)) + ((- 1))) 0))).[e_state_s_granule] :<
+                  0)))));
+      (Some (0, st_7)))
+    else (
+      when st_5 == (
+          (granule_unlock_spec
+            (mkPtr "granules" (v_0_abs.(meta_granule_offset)))
+            (st_1.[share].[globals].[g_granules] :<
+              ((((st_1.(share)).(globals)).(g_granules)) #
+                ((v_0_abs.(meta_granule_offset)) / (16)) ==
+                (((((st_1.(share)).(globals)).(g_granules)) @ ((v_0_abs.(meta_granule_offset)) / (16))).[e_ref] :<
+                  ((((((st_1.(share)).(globals)).(g_granules)) @ ((v_0_abs.(meta_granule_offset)) / (16))).(e_ref)).[e_u_anon_3_0] :<
+                    (g_mapped_addr_set_para (((((((st_1.(share)).(globals)).(g_granules)) @ ((v_0_abs.(meta_granule_offset)) / (16))).(e_ref)).(e_u_anon_3_0)) + ((- 1))) 0)))))));
+      (Some (0, st_5))))
+  else (
+    when st_2 == ((spinlock_release_spec (mkPtr "granules" (v_0_abs.(meta_granule_offset))) st_1));
+    (Some ((pack_struct_return_code_para (make_return_code_para 1)), st_2))).
+
+Definition s1tte_is_valid_spec (v_0: Z) (v_1: Z) (st: RData) : (option (bool * RData)) :=
+  if ((v_1 =? (3)) && (((v_0 & (3)) =? (3))))
+  then (Some (true, st))
+  else (
+    if ((v_1 <>? (3)) && (((v_0 & (3)) =? (1))))
+    then (Some (true, st))
+    else (Some (false, st))).
+
+Definition smc_granule_ns_to_any_spec (v_0: Z) (st: RData) : (option (Z * RData)) :=
+  None.
+
+Definition smc_granule_any_to_ns_spec (v_0: Z) (st: RData) : (option (Z * RData)) :=
   None.
 
