container/coq/pointer/.CachedSpec/Layer3Spec.v
@@ -80,52 +80,10 @@ Definition entry_is_table_spec (v_0: Z) (st: RData) : (option (bool * RData)) :=
   (Some (((v_0 & (3)) =? (3)), st)).
 
 Definition granule_try_lock_spec (v_0: Ptr) (v_1: Z) (st: RData) : (option (bool * RData)) :=
-  when st_0 == (
-      if ((v_0.(pbase)) =s ("granules"))
-      then (
-        match (((((((st.(share)).(globals)).(g_granules)) @ ((v_0.(poffset)) / (16))).(e_lock)).(e_val))) with
-        | None =>
-          rely (
-            (((((((st.(share)).(globals)).(g_granules)) @ ((v_0.(poffset)) / (16))).(e_state_s_granule)) -
-              ((((((st.(share)).(globals)).(g_granules)) @ ((v_0.(poffset)) / (16))).(e_state_s_granule)))) =
-              (0)));
-          (Some ((st.[log] :< ((EVT CPU_ID (ACQ ((v_0.(poffset)) / (16)))) :: ((st.(log))))).[share].[globals].[g_granules] :<
-            ((((st.(share)).(globals)).(g_granules)) #
-              ((v_0.(poffset)) / (16)) ==
-              (((((st.(share)).(globals)).(g_granules)) @ ((v_0.(poffset)) / (16))).[e_lock].[e_val] :< (Some CPU_ID)))))
-        | (Some cid) => None
-        end)
-      else (
-        if ((v_0.(pbase)) =s ("vmid_lock"))
-        then (
-          match (
-            if ((v_0.(poffset)) =? (0))
-            then ((((st.(share)).(globals)).(g_vmid_lock)).(e_val))
-            else None
-          ) with
-          | None => (Some ((st.[log] :< ((EVT CPU_ID (ACQ vmid_lock_idx)) :: ((st.(log))))).[share].[globals].[g_vmid_lock].[e_val] :< (Some CPU_ID)))
-          | (Some cid) => None
-          end)
-        else None));
+  when st_0 == ((spinlock_acquire_spec (mkPtr (v_0.(pbase)) (v_0.(poffset))) st));
   if (((((((st_0.(share)).(globals)).(g_granules)) @ ((v_0.(poffset)) / (16))).(e_state_s_granule)) - (v_1)) =? (0))
   then (Some (true, st_0))
   else (
-    when st_2 == (
-        if ((v_0.(pbase)) =s ("granules"))
-        then (
-          when cid == (((((((st_0.(share)).(globals)).(g_granules)) @ ((v_0.(poffset)) / (16))).(e_lock)).(e_val)));
-          (Some ((st_0.[log] :< ((EVT CPU_ID (REL ((v_0.(poffset)) / (16)) ((((st_0.(share)).(globals)).(g_granules)) @ ((v_0.(poffset)) / (16))))) :: ((st_0.(log))))).[share].[globals].[g_granules] :<
-            ((((st_0.(share)).(globals)).(g_granules)) #
-              ((v_0.(poffset)) / (16)) ==
-              (((((st_0.(share)).(globals)).(g_granules)) @ ((v_0.(poffset)) / (16))).[e_lock].[e_val] :< None)))))
-        else (
-          if ((v_0.(pbase)) =s ("vmid_lock"))
-          then (
-            when cid == (
-                if ((v_0.(poffset)) =? (0))
-                then ((((st_0.(share)).(globals)).(g_vmid_lock)).(e_val))
-                else None);
-            (Some ((st_0.[log] :< ((EVT CPU_ID (REL vmid_lock_idx vmid_lock_g)) :: ((st_0.(log))))).[share].[globals].[g_vmid_lock].[e_val] :< None)))
-          else None));
+    when st_2 == ((spinlock_release_spec (mkPtr (v_0.(pbase)) (v_0.(poffset))) st_0));
     (Some (false, st_2))).
 
