container/coq/pointer/.CachedSpec/Layer5Spec.v
@@ -6,6 +6,9 @@ Parameter memcpy_ns_read_spec_state_oracle : Ptr -> (Ptr -> (Z -> (RData -> (opt
 
 Parameter monitor_call_state_oracle : Z -> (Z -> (Z -> (Z -> (Z -> (Z -> (Z -> (RData -> (option (Z * RData))))))))).
 
+Definition s2tte_create_unassigned_spec_abs (v_0: Z) (st: RData) : (option (abs_PTE_t * RData)) :=
+  (Some ((mkabs_PTE_t (mkabs_PA_t (- 1)) 0 v_0), st)).
+
 Definition llvm_memset_p0i8_i64_spec (v_0: Ptr) (arg1: Z) (arg2: Z) (arg3: bool) (st: RData) : (option RData) :=
   when st_0 == ((llvm_memset_p0i8_i64_spec_state_oracle v_0 arg1 arg2 arg3 st));
   rely ((((st_0.(share)).(granule_data)) = (((st.(share)).(granule_data)))));
@@ -48,27 +51,8 @@ Definition atomic_add_64 (loc: Ptr) (val: Z) (st: RData) : (option RData) :=
   when st_2 == ((store_RData_granules 64 loc (v + (val)) st_1));
   (Some st_2).
 
-Definition s2tte_is_table_spec (v_0: Z) (v_1: Z) (st: RData) : (option (bool * RData)) :=
-  (Some (((v_1 <? (3)) && (((v_0 & (3)) =? (3)))), st)).
-
 Definition granule_unlock_spec (v_0: Ptr) (st: RData) : (option RData) :=
-  when st_0 == (
-      if ((v_0.(pbase)) =s ("granules"))
-      then (
-        when cid == (((((((st.(share)).(globals)).(g_granules)) @ ((v_0.(poffset)) / (16))).(e_lock)).(e_val)));
-        (Some ((st.[log] :< ((EVT CPU_ID (REL ((v_0.(poffset)) / (16)) ((((st.(share)).(globals)).(g_granules)) @ ((v_0.(poffset)) / (16))))) :: ((st.(log))))).[share].[globals].[g_granules] :<
-          ((((st.(share)).(globals)).(g_granules)) #
-            ((v_0.(poffset)) / (16)) ==
-            (((((st.(share)).(globals)).(g_granules)) @ ((v_0.(poffset)) / (16))).[e_lock].[e_val] :< None)))))
-      else (
-        if ((v_0.(pbase)) =s ("vmid_lock"))
-        then (
-          when cid == (
-              if ((v_0.(poffset)) =? (0))
-              then ((((st.(share)).(globals)).(g_vmid_lock)).(e_val))
-              else None);
-          (Some ((st.[log] :< ((EVT CPU_ID (REL vmid_lock_idx vmid_lock_g)) :: ((st.(log))))).[share].[globals].[g_vmid_lock].[e_val] :< None)))
-        else None));
+  when st_0 == ((spinlock_release_spec (mkPtr (v_0.(pbase)) (v_0.(poffset))) st));
   (Some st_0).
 
 Definition s2_sl_addr_to_idx_spec (v_0: Z) (v_1: Z) (v_2: Z) (st: RData) : (option (Z * RData)) :=
@@ -95,61 +79,30 @@ Definition make_return_code_spec (v_0: Z) (v_1: Z) (st: RData) : (option (Z * RD
   (Some ((make_return_code_para v_0), st)).
 
 Definition atomic_granule_get_spec (v_0: Ptr) (st: RData) : (option RData) :=
-  when st_0 == (
-      rely (((v_0.(pbase)) =s ("granules")));
-      rely (((((v_0.(poffset)) + (8)) mod (16)) = (8)));
-      when v, st_1 == (
-          when ret == (
-              if (((((v_0.(poffset)) + (8)) mod (16)) >=? (0)) && (((((v_0.(poffset)) + (8)) mod (16)) <? (4))))
-              then (
-                if ((((v_0.(poffset)) + (8)) mod (16)) =? (0))
-                then ((((((st.(share)).(globals)).(g_granules)) @ (((v_0.(poffset)) + (8)) / (16))).(e_lock)).(e_val))
-                else None)
-              else (
-                if ((((v_0.(poffset)) + (8)) mod (16)) =? (4))
-                then (Some (((((st.(share)).(globals)).(g_granules)) @ (((v_0.(poffset)) + (8)) / (16))).(e_state_s_granule)))
-                else (
-                  if (((((v_0.(poffset)) + (8)) mod (16)) >=? (8)) && (((((v_0.(poffset)) + (8)) mod (16)) <? (16))))
-                  then (
-                    if (((((v_0.(poffset)) + (8)) mod (16)) - (8)) =? (0))
-                    then (Some ((((((st.(share)).(globals)).(g_granules)) @ (((v_0.(poffset)) + (8)) / (16))).(e_ref)).(e_u_anon_3_0)))
-                    else None)
-                  else None)));
-          (Some (ret, st)));
-      when st_2 == (
-          when ret == (
-              if (((((v_0.(poffset)) + (8)) mod (16)) >=? (0)) && (((((v_0.(poffset)) + (8)) mod (16)) <? (4))))
-              then (
-                when ret == (
-                    if ((((v_0.(poffset)) + (8)) mod (16)) =? (0))
-                    then (Some ((((((st_1.(share)).(globals)).(g_granules)) @ (((v_0.(poffset)) + (8)) / (16))).(e_lock)).[e_val] :< (Some (v + (1)))))
-                    else None);
-                (Some (((((st_1.(share)).(globals)).(g_granules)) @ (((v_0.(poffset)) + (8)) / (16))).[e_lock] :< ret)))
-              else (
-                if ((((v_0.(poffset)) + (8)) mod (16)) =? (4))
-                then (Some (((((st_1.(share)).(globals)).(g_granules)) @ (((v_0.(poffset)) + (8)) / (16))).[e_state_s_granule] :< (v + (1))))
-                else (
-                  if (((((v_0.(poffset)) + (8)) mod (16)) >=? (8)) && (((((v_0.(poffset)) + (8)) mod (16)) <? (16))))
-                  then (
-                    when ret == (
-                        if (((((v_0.(poffset)) + (8)) mod (16)) - (8)) =? (0))
-                        then (Some ((((((st_1.(share)).(globals)).(g_granules)) @ (((v_0.(poffset)) + (8)) / (16))).(e_ref)).[e_u_anon_3_0] :< (v + (1))))
-                        else None);
-                    (Some (((((st_1.(share)).(globals)).(g_granules)) @ (((v_0.(poffset)) + (8)) / (16))).[e_ref] :< ret)))
-                  else None)));
-          (Some (st_1.[share].[globals].[g_granules] :< ((((st_1.(share)).(globals)).(g_granules)) # (((v_0.(poffset)) + (8)) / (16)) == ret))));
-      (Some st_2));
-  (Some st_0).
+  rely (((v_0.(pbase)) =s ("granules")));
+  rely (((((v_0.(poffset)) + (8)) mod (16)) = (8)));
+  (Some (st.[share].[globals].[g_granules] :<
+    ((((st.(share)).(globals)).(g_granules)) #
+      (((v_0.(poffset)) + (8)) / (16)) ==
+      (((((st.(share)).(globals)).(g_granules)) @ (((v_0.(poffset)) + (8)) / (16))).[e_ref] :<
+        ((((((st.(share)).(globals)).(g_granules)) @ (((v_0.(poffset)) + (8)) / (16))).(e_ref)).[e_u_anon_3_0] :<
+          (((((((st.(share)).(globals)).(g_granules)) @ (((v_0.(poffset)) + (8)) / (16))).(e_ref)).(e_u_anon_3_0)) + (1))))))).
+
+Definition atomic_granule_put_spec (v_0: Ptr) (st: RData) : (option RData) :=
+  rely (((v_0.(pbase)) =s ("granules")));
+  rely (((((v_0.(poffset)) + (8)) mod (16)) = (8)));
+  (Some (st.[share].[globals].[g_granules] :<
+    ((((st.(share)).(globals)).(g_granules)) #
+      (((v_0.(poffset)) + (8)) / (16)) ==
+      (((((st.(share)).(globals)).(g_granules)) @ (((v_0.(poffset)) + (8)) / (16))).[e_ref] :<
+        ((((((st.(share)).(globals)).(g_granules)) @ (((v_0.(poffset)) + (8)) / (16))).(e_ref)).[e_u_anon_3_0] :<
+          (((((((st.(share)).(globals)).(g_granules)) @ (((v_0.(poffset)) + (8)) / (16))).(e_ref)).(e_u_anon_3_0)) + ((- 1)))))))).
 
 Definition find_lock_granule_spec (v_0: abs_PA_t) (v_1: Z) (st: RData) : (option (Ptr * RData)) :=
   None.
 
 Definition s2tte_create_unassigned_spec (v_0: Z) (st: RData) : (option (Z * RData)) :=
-  when v_2, st_0 == (
-      when v__0, st_1 == (
-          if (v_0 =? (0))
-          then (Some (0, st))
-          else (Some (64, st)));
-      (Some (v__0, st_1)));
-  (Some (v_2, st_0)).
+  if (v_0 =? (0))
+  then (Some (0, st))
+  else (Some (64, st)).
 
