container/coq/pointer/Layer1/buffer_map/LowSpec.v
@@ -11,11 +11,9 @@ Section Layer1_buffer_map_LowSpec.
   Context `{int_ptr: IntPtrCast}.
 
   Definition buffer_map_spec_low (v_0: Z) (v_1: Z) (v_2: bool) (st: RData) : (option (Ptr * RData)) :=
-    when v__0_in, st_0 == (
-        if ((v_1 & (549755813888)) =? (0))
-        then (Some ((v_1 + (18446744004990074880)), st))
-        else (Some ((v_1 + (18446743457381744640)), st)));
-    (Some ((int_to_ptr v__0_in), st_0)).
+    if ((v_1 & (549755813888)) =? (0))
+    then (Some ((int_to_ptr (v_1 + (18446744004990074880))), st))
+    else (Some ((int_to_ptr (v_1 + (18446743457381744640))), st)).
 
 End Layer1_buffer_map_LowSpec.
 
