container/coq/pointer/Layer1/granule_addr/LowSpec.v
@@ -11,11 +11,9 @@ Section Layer1_granule_addr_LowSpec.
   Context `{int_ptr: IntPtrCast}.
 
   Definition granule_addr_spec_low (v_0: Ptr) (st: RData) : (option (Z * RData)) :=
-    when v__0, st_0 == (
-        if (((ptr_to_int v_0) - ((ptr_to_int (mkPtr "granules" 0)))) >? (8388592))
-        then (Some (((((ptr_to_int v_0) - ((ptr_to_int (mkPtr "granules" 0)))) * (256)) + (549755813888)), st))
-        else (Some (((((ptr_to_int v_0) - ((ptr_to_int (mkPtr "granules" 0)))) * (256)) + (2147483648)), st)));
-    (Some (v__0, st_0)).
+    if (((ptr_to_int v_0) - ((ptr_to_int (mkPtr "granules" 0)))) >? (8388592))
+    then (Some (((((ptr_to_int v_0) - ((ptr_to_int (mkPtr "granules" 0)))) * (256)) + (549755813888)), st))
+    else (Some (((((ptr_to_int v_0) - ((ptr_to_int (mkPtr "granules" 0)))) * (256)) + (2147483648)), st)).
 
 End Layer1_granule_addr_LowSpec.
 
