container/coq/pointer/Layer2/addr_level_mask/LowSpec.v
@@ -11,7 +11,7 @@ Section Layer2_addr_level_mask_LowSpec.
   Context `{int_ptr: IntPtrCast}.
 
   Definition addr_level_mask_spec_low (v_0: Z) (v_1: Z) (st: RData) : (option (Z * RData)) :=
-    (Some (((v_0 & (281474976710655)) & (((- 1) << (((((3 - (v_1)) * (9)) + (12)) & (4294967295)))))), st)).
+    (Some (((v_0 & (281474976710655)) & (((- 1) << (((39 + (((- 9) * (v_1)))) & (4294967295)))))), st)).
 
 End Layer2_addr_level_mask_LowSpec.
 
