container/coq/pointer/Layer2/addr_to_idx/LowSpec.v
@@ -11,12 +11,10 @@ Section Layer2_addr_to_idx_LowSpec.
   Context `{int_ptr: IntPtrCast}.
 
   Definition addr_to_idx_spec_low (v_0: Z) (st: RData) : (option (Z * RData)) :=
-    rely (((((v_0 - (MEM0_PHYS)) >= (0)) /\ (((v_0 - ((MEM0_PHYS + (MEM0_SIZE)))) < (0)))) \/ ((((v_0 - (MEM1_PHYS)) >= (0)) /\ (((v_0 - ((MEM1_PHYS + (MEM1_SIZE)))) < (0)))))));
-    when v__0, st_0 == (
-        if (v_0 >? (551903297535))
-        then (Some ((((v_0 + (18446743521806254080)) >> (12)) + (524288)), st))
-        else (Some (((v_0 + (18446744071562067968)) >> (12)), st)));
-    (Some (v__0, st_0)).
+    rely (((((v_0 - (MEM0_PHYS)) >= (0)) /\ (((v_0 - (4294967296)) < (0)))) \/ ((((v_0 - (MEM1_PHYS)) >= (0)) /\ (((v_0 - (556198264832)) < (0)))))));
+    if (v_0 >? (551903297535))
+    then (Some ((((v_0 + (18446743521806254080)) >> (12)) + (524288)), st))
+    else (Some (((v_0 + (18446744071562067968)) >> (12)), st)).
 
 End Layer2_addr_to_idx_LowSpec.
 
