container/coq/pointer/Layer3/Spec.v
@@ -92,60 +92,18 @@ Section Layer3_Spec.
     (Some (((v_0 & (3)) =? (3)), st)).
 
   Definition granule_try_lock_spec (v_0: Ptr) (v_1: Z) (st: RData) : (option (bool * RData)) :=
-    when st_0 == (
-        if ((v_0.(pbase)) =s ("granules"))
-        then (
-          match (((((((st.(share)).(globals)).(g_granules)) @ ((v_0.(poffset)) / (16))).(e_lock)).(e_val))) with
-          | None =>
-            rely (
-              (((((((st.(share)).(globals)).(g_granules)) @ ((v_0.(poffset)) / (16))).(e_state_s_granule)) -
-                ((((((st.(share)).(globals)).(g_granules)) @ ((v_0.(poffset)) / (16))).(e_state_s_granule)))) =
-                (0)));
-            (Some ((st.[log] :< ((EVT CPU_ID (ACQ ((v_0.(poffset)) / (16)))) :: ((st.(log))))).[share].[globals].[g_granules] :<
-              ((((st.(share)).(globals)).(g_granules)) #
-                ((v_0.(poffset)) / (16)) ==
-                (((((st.(share)).(globals)).(g_granules)) @ ((v_0.(poffset)) / (16))).[e_lock].[e_val] :< (Some CPU_ID)))))
-          | (Some cid) => None
-          end)
-        else (
-          if ((v_0.(pbase)) =s ("vmid_lock"))
-          then (
-            match (
-              if ((v_0.(poffset)) =? (0))
-              then ((((st.(share)).(globals)).(g_vmid_lock)).(e_val))
-              else None
-            ) with
-            | None => (Some ((st.[log] :< ((EVT CPU_ID (ACQ vmid_lock_idx)) :: ((st.(log))))).[share].[globals].[g_vmid_lock].[e_val] :< (Some CPU_ID)))
-            | (Some cid) => None
-            end)
-          else None));
+    when st_0 == ((spinlock_acquire_spec (mkPtr (v_0.(pbase)) (v_0.(poffset))) st));
     if (((((((st_0.(share)).(globals)).(g_granules)) @ ((v_0.(poffset)) / (16))).(e_state_s_granule)) - (v_1)) =? (0))
     then (Some (true, st_0))
     else (
-      when st_2 == (
-          if ((v_0.(pbase)) =s ("granules"))
-          then (
-            when cid == (((((((st_0.(share)).(globals)).(g_granules)) @ ((v_0.(poffset)) / (16))).(e_lock)).(e_val)));
-            (Some ((st_0.[log] :< ((EVT CPU_ID (REL ((v_0.(poffset)) / (16)) ((((st_0.(share)).(globals)).(g_granules)) @ ((v_0.(poffset)) / (16))))) :: ((st_0.(log))))).[share].[globals].[g_granules] :<
-              ((((st_0.(share)).(globals)).(g_granules)) #
-                ((v_0.(poffset)) / (16)) ==
-                (((((st_0.(share)).(globals)).(g_granules)) @ ((v_0.(poffset)) / (16))).[e_lock].[e_val] :< None)))))
-          else (
-            if ((v_0.(pbase)) =s ("vmid_lock"))
-            then (
-              when cid == (
-                  if ((v_0.(poffset)) =? (0))
-                  then ((((st_0.(share)).(globals)).(g_vmid_lock)).(e_val))
-                  else None);
-              (Some ((st_0.[log] :< ((EVT CPU_ID (REL vmid_lock_idx vmid_lock_g)) :: ((st_0.(log))))).[share].[globals].[g_vmid_lock].[e_val] :< None)))
-            else None));
+      when st_2 == ((spinlock_release_spec (mkPtr (v_0.(pbase)) (v_0.(poffset))) st_0));
       (Some (false, st_2))).
 
 End Layer3_Spec.
 
 #[global] Hint Unfold addr_to_granule_spec_abs: spec.
-#[global] Hint Unfold spinlock_release_spec: spec.
-#[global] Hint Unfold spinlock_acquire_spec: spec.
+Opaque spinlock_release_spec.
+Opaque spinlock_acquire_spec.
 #[global] Hint Unfold block_granule_try_lock_spec: spec.
 #[global] Hint Unfold __table_get_entry_spec_abs: spec.
 #[global] Hint Unfold entry_is_table_spec_abs: spec.
@@ -154,4 +112,4 @@ End Layer3_Spec.
 #[global] Hint Unfold addr_to_granule_spec: spec.
 #[global] Hint Unfold __table_get_entry_spec: spec.
 #[global] Hint Unfold entry_is_table_spec: spec.
-Opaque granule_try_lock_spec.
+#[global] Hint Unfold granule_try_lock_spec: spec.
