container/coq/pointer/Layer5/atomic_granule_put/LowSpec.v
@@ -2,7 +2,6 @@ Require Import Code.
 Require Import CommonDeps.
 Require Import DataTypes.
 Require Import GlobalDefs.
-Require Import Layer4.Spec.
 
 Local Open Scope string_scope.
 Local Open Scope Z_scope.
@@ -12,10 +11,8 @@ Section Layer5_atomic_granule_put_LowSpec.
   Context `{int_ptr: IntPtrCast}.
 
   Definition atomic_granule_put_spec_low (v_0: Ptr) (st: RData) : (option RData) :=
-    rely (((((v_0.(pbase)) = ("granules")) /\ ((((v_0.(poffset)) mod (16)) = (0)))) /\ (((v_0.(poffset)) >= (0)))));
-    when v, st_1 == ((load_RData 64 (mkPtr (v_0.(pbase)) ((v_0.(poffset)) + (8))) st));
-    when st_2 == ((store_RData 64 (mkPtr (v_0.(pbase)) ((v_0.(poffset)) + (8))) (v + ((- 1))) st_1));
-    (Some st_2).
+    when st_0 == ((atomic_add_64 (ptr_offset v_0 8) (- 1) st));
+    (Some st_0).
 
 End Layer5_atomic_granule_put_LowSpec.
 
