container/coq/pointer/Layer6/g_mapped_addr_set/LowSpec.v
@@ -12,8 +12,8 @@ Section Layer6_g_mapped_addr_set_LowSpec.
 
   Definition g_mapped_addr_set_spec_low (v_0: Ptr) (v_1: Z) (st: RData) : (option RData) :=
     rely (((((v_0.(pbase)) = ("granules")) /\ ((((v_0.(poffset)) mod (16)) = (0)))) /\ (((v_0.(poffset)) >= (0)))));
-    when v_4, st_0 == ((load_RData 8 (mkPtr (v_0.(pbase)) ((v_0.(poffset)) + (8))) st));
-    when st_1 == ((store_RData 8 (mkPtr (v_0.(pbase)) ((v_0.(poffset)) + (8))) ((v_4 & (4095)) |' (v_1)) st_0));
+    when v_4, st_0 == ((load_RData 8 (ptr_offset v_0 8) st));
+    when st_1 == ((store_RData 8 (ptr_offset v_0 8) ((v_4 & (4095)) |' (v_1)) st_0));
     (Some st_1).
 
 End Layer6_g_mapped_addr_set_LowSpec.
