container/coq/pointer/Layer6/g_refcount/LowSpec.v
@@ -12,7 +12,7 @@ Section Layer6_g_refcount_LowSpec.
 
   Definition g_refcount_spec_low (v_0: Ptr) (st: RData) : (option (Z * RData)) :=
     rely (((((v_0.(pbase)) = ("granules")) /\ ((((v_0.(poffset)) mod (16)) = (0)))) /\ (((v_0.(poffset)) >= (0)))));
-    when v_3, st_0 == ((load_RData 8 (mkPtr (v_0.(pbase)) ((v_0.(poffset)) + (8))) st));
+    when v_3, st_0 == ((load_RData 8 (ptr_offset v_0 8) st));
     (Some ((v_3 & (4095)), st_0)).
 
 End Layer6_g_refcount_LowSpec.
