container/coq/pointer/Layer7/smc_granule_any_to_ns/LowSpec.v
@@ -1,0 +1,18 @@
+Require Import Code.
+Require Import CommonDeps.
+Require Import DataTypes.
+Require Import GlobalDefs.
+
+Local Open Scope string_scope.
+Local Open Scope Z_scope.
+
+Section Layer7_smc_granule_any_to_ns_LowSpec.
+
+  Context `{int_ptr: IntPtrCast}.
+
+  Definition smc_granule_any_to_ns_spec_low (v_0: Z) (st: RData) : (option (Z * RData)) :=
+    None.
+
+End Layer7_smc_granule_any_to_ns_LowSpec.
+
+#[global] Hint Unfold smc_granule_any_to_ns_spec_low: spec.
