container/coq/pointer/Layer8/Spec.v
@@ -23,230 +23,504 @@ Section Layer8_Spec.
     when v_7, st_2 == ((rtt_create_internal_spec_abs ttbr v_1 v_2 v_3 1 st_1));
     ((Some v_7), st_2).
 
-  Definition rtt_create_s1_el1_spec (v_0: Ptr) (v_1: Z) (v_2: Z) (v_3: Z) (st: RData) : (option (Z * RData)) :=
-    when st_1 == ((granule_lock_spec (rec_to_ttbr1_para v_0 st) 5 st));
-    when v_7, st_2 == (
-        when ret, st' == ((granule_try_lock_spec (mkPtr "granules" ((test_PA v_1).(meta_granule_offset))) 1 st_1));
-        if ret
+  Definition map_unmap_ns_s1_0 (st_0: RData) (st_12: RData) (v_17: Ptr) (v_3: abs_PTE_t) (v_31: Z) (v__sroa_0_0_copyload: Ptr) (v__sroa_7_0_copyload: Z) : (option (Z * RData)) :=
+    rely (((v_31 =? (0)) = (true)));
+    rely (((v__sroa_0_0_copyload.(pbase)) =s ("granules")));
+    rely (((((v__sroa_0_0_copyload.(poffset)) + (8)) mod (16)) = (8)));
+    when st_19 == (
+        (granule_unlock_spec
+          v__sroa_0_0_copyload
+          ((st_12.[share].[globals].[g_granules] :<
+            ((((st_12.(share)).(globals)).(g_granules)) #
+              (((v__sroa_0_0_copyload.(poffset)) + (8)) / (16)) ==
+              (((((st_12.(share)).(globals)).(g_granules)) @ (((v__sroa_0_0_copyload.(poffset)) + (8)) / (16))).[e_ref] :<
+                ((((((st_12.(share)).(globals)).(g_granules)) @ (((v__sroa_0_0_copyload.(poffset)) + (8)) / (16))).(e_ref)).[e_u_anon_3_0] :<
+                  (((((((st_12.(share)).(globals)).(g_granules)) @ (((v__sroa_0_0_copyload.(poffset)) + (8)) / (16))).(e_ref)).(e_u_anon_3_0)) + (1)))))).[share].[granule_data] :<
+            (((st_12.(share)).(granule_data)) #
+              (((v_17.(poffset)) + ((8 * (v__sroa_7_0_copyload)))) / (4096)) ==
+              ((((st_12.(share)).(granule_data)) @ (((v_17.(poffset)) + ((8 * (v__sroa_7_0_copyload)))) / (4096))).[g_norm] :<
+                (((((st_12.(share)).(granule_data)) @ (((v_17.(poffset)) + ((8 * (v__sroa_7_0_copyload)))) / (4096))).(g_norm)) #
+                  (((v_17.(poffset)) + ((8 * (v__sroa_7_0_copyload)))) mod (4096)) ==
+                  (test_PTE_Z v_3)))))));
+    (Some (0, st_19)).
+
+  Definition map_unmap_ns_s1_1 (st_0: RData) (st_11: RData) (v_17: Ptr) (v_3: abs_PTE_t) (v__sroa_0_0_copyload: Ptr) (v__sroa_7_0_copyload: Z) : (option (Z * RData)) :=
+    rely (((v__sroa_0_0_copyload.(pbase)) =s ("granules")));
+    rely (((((v__sroa_0_0_copyload.(poffset)) + (8)) mod (16)) = (8)));
+    when st_18 == (
+        (granule_unlock_spec
+          v__sroa_0_0_copyload
+          ((st_11.[share].[globals].[g_granules] :<
+            ((((st_11.(share)).(globals)).(g_granules)) #
+              (((v__sroa_0_0_copyload.(poffset)) + (8)) / (16)) ==
+              (((((st_11.(share)).(globals)).(g_granules)) @ (((v__sroa_0_0_copyload.(poffset)) + (8)) / (16))).[e_ref] :<
+                ((((((st_11.(share)).(globals)).(g_granules)) @ (((v__sroa_0_0_copyload.(poffset)) + (8)) / (16))).(e_ref)).[e_u_anon_3_0] :<
+                  (((((((st_11.(share)).(globals)).(g_granules)) @ (((v__sroa_0_0_copyload.(poffset)) + (8)) / (16))).(e_ref)).(e_u_anon_3_0)) + (1)))))).[share].[granule_data] :<
+            (((st_11.(share)).(granule_data)) #
+              (((v_17.(poffset)) + ((8 * (v__sroa_7_0_copyload)))) / (4096)) ==
+              ((((st_11.(share)).(granule_data)) @ (((v_17.(poffset)) + ((8 * (v__sroa_7_0_copyload)))) / (4096))).[g_norm] :<
+                (((((st_11.(share)).(granule_data)) @ (((v_17.(poffset)) + ((8 * (v__sroa_7_0_copyload)))) / (4096))).(g_norm)) #
+                  (((v_17.(poffset)) + ((8 * (v__sroa_7_0_copyload)))) mod (4096)) ==
+                  (test_PTE_Z v_3)))))));
+    (Some (0, st_18)).
+
+  Definition map_unmap_ns_s1_2 (st_0: RData) (st_12: RData) (v_17: Ptr) (v_47: Z) (v__sroa_0_0_copyload: Ptr) (v__sroa_7_0_copyload: Z) : (option (Z * RData)) :=
+    rely (((v_47 =? (0)) = (true)));
+    rely (((((v__sroa_0_0_copyload.(pbase)) = ("granules")) /\ ((((v__sroa_0_0_copyload.(poffset)) mod (16)) = (0)))) /\ (((v__sroa_0_0_copyload.(poffset)) >= (0)))));
+    when st_20 == (
+        (granule_unlock_spec
+          v__sroa_0_0_copyload
+          ((st_12.[share].[globals].[g_granules] :<
+            ((((st_12.(share)).(globals)).(g_granules)) #
+              ((v__sroa_0_0_copyload.(poffset)) / (16)) ==
+              (((((st_12.(share)).(globals)).(g_granules)) @ ((v__sroa_0_0_copyload.(poffset)) / (16))).[e_ref] :<
+                ((((((st_12.(share)).(globals)).(g_granules)) @ ((v__sroa_0_0_copyload.(poffset)) / (16))).(e_ref)).[e_u_anon_3_0] :<
+                  (((((((st_12.(share)).(globals)).(g_granules)) @ ((v__sroa_0_0_copyload.(poffset)) / (16))).(e_ref)).(e_u_anon_3_0)) + ((- 1))))))).[share].[granule_data] :<
+            (((st_12.(share)).(granule_data)) #
+              (((v_17.(poffset)) + ((8 * (v__sroa_7_0_copyload)))) / (4096)) ==
+              ((((st_12.(share)).(granule_data)) @ (((v_17.(poffset)) + ((8 * (v__sroa_7_0_copyload)))) / (4096))).[g_norm] :<
+                (((((st_12.(share)).(granule_data)) @ (((v_17.(poffset)) + ((8 * (v__sroa_7_0_copyload)))) / (4096))).(g_norm)) #
+                  (((v_17.(poffset)) + ((8 * (v__sroa_7_0_copyload)))) mod (4096)) ==
+                  (test_PTE_Z (mkabs_PTE_t (mkabs_PA_t (- 1)) 0 1))))))));
+    (Some (0, st_20)).
+
+  Definition map_unmap_ns_s1_3 (st_0: RData) (st_11: RData) (v_17: Ptr) (v_20: abs_PTE_t) (v__sroa_0_0_copyload: Ptr) (v__sroa_7_0_copyload: Z) : (option (Z * RData)) :=
+    rely (((((v__sroa_0_0_copyload.(pbase)) = ("granules")) /\ ((((v__sroa_0_0_copyload.(poffset)) mod (16)) = (0)))) /\ (((v__sroa_0_0_copyload.(poffset)) >= (0)))));
+    when st_19 == (
+        (granule_unlock_spec
+          v__sroa_0_0_copyload
+          ((st_11.[share].[globals].[g_granules] :<
+            ((((st_11.(share)).(globals)).(g_granules)) #
+              ((v__sroa_0_0_copyload.(poffset)) / (16)) ==
+              (((((st_11.(share)).(globals)).(g_granules)) @ ((v__sroa_0_0_copyload.(poffset)) / (16))).[e_ref] :<
+                ((((((st_11.(share)).(globals)).(g_granules)) @ ((v__sroa_0_0_copyload.(poffset)) / (16))).(e_ref)).[e_u_anon_3_0] :<
+                  (((((((st_11.(share)).(globals)).(g_granules)) @ ((v__sroa_0_0_copyload.(poffset)) / (16))).(e_ref)).(e_u_anon_3_0)) + ((- 1))))))).[share].[granule_data] :<
+            (((st_11.(share)).(granule_data)) #
+              (((v_17.(poffset)) + ((8 * (v__sroa_7_0_copyload)))) / (4096)) ==
+              ((((st_11.(share)).(granule_data)) @ (((v_17.(poffset)) + ((8 * (v__sroa_7_0_copyload)))) / (4096))).[g_norm] :<
+                (((((st_11.(share)).(granule_data)) @ (((v_17.(poffset)) + ((8 * (v__sroa_7_0_copyload)))) / (4096))).(g_norm)) #
+                  (((v_17.(poffset)) + ((8 * (v__sroa_7_0_copyload)))) mod (4096)) ==
+                  (test_PTE_Z (mkabs_PTE_t (mkabs_PA_t (- 1)) 0 1))))))));
+    (Some (0, st_19)).
+
+  Definition map_unmap_ns_s1_spec (v_0_Zptr: Z) (v_1: Z) (v_2: Z) (v_3: Z) (v_4: Z) (st: RData) : (option (Z * RData)) :=
+    when st_3 == ((granule_lock_spec (mkPtr "granules" ((test_PA v_0_Zptr).(meta_granule_offset))) 5 st));
+    when ret_rtt, st_4 == ((rtt_walk_lock_unlock_spec_abs (mkPtr "stack_s_rtt_walk" 0) (mkPtr "granules" ((test_PA v_0_Zptr).(meta_granule_offset))) 0 64 v_1 v_2 st_3));
+    rely ((((st_4.(share)).(granule_data)) = (((st_3.(share)).(granule_data)))));
+    if (((ret_rtt.(e_1)) - (v_2)) =? (0))
+    then (
+      if (v_4 =? (0))
+      then (
+        if (
+          ((((abs_tte_read (mkPtr "granule_data" (((ret_rtt.(e_2)).(poffset)) + ((8 * ((ret_rtt.(e_3))))))) st_4).(meta_desc_type)) =? (0)) &&
+            ((((abs_tte_read (mkPtr "granule_data" (((ret_rtt.(e_2)).(poffset)) + ((8 * ((ret_rtt.(e_3))))))) st_4).(meta_ripas)) =? (0)))))
         then (
-          when ret_record, st_4 == ((rtt_walk_lock_unlock_spec_abs (mkPtr "stack_s_rtt_walk" 0) (rec_to_ttbr1_para v_0 st) 0 64 v_2 v_3 st'));
-          rely ((((ret_record.(e_2)).(pbase)) =s ("granules")));
-          rely (((((ret_record.(e_2)).(poffset)) mod (16)) = (0)));
-          rely ((((ret_record.(e_1)) <= (3)) /\ (((ret_record.(e_1)) >= (0)))));
-          if (((ret_record.(e_1)) - ((v_3 + ((- 1))))) =? (0))
+          if (uart0_phys_para (test_Z_PTE v_3))
           then (
-            if (
-              ((((abs_tte_read (mkPtr "granule_data" (((ret_record.(e_2)).(poffset)) + ((8 * ((ret_record.(e_3))))))) st_4).(meta_desc_type)) =? (0)) &&
-                ((((abs_tte_read (mkPtr "granule_data" (((ret_record.(e_2)).(poffset)) + ((8 * ((ret_record.(e_3))))))) st_4).(meta_ripas)) =? (0)))))
+            rely ((((ret_rtt.(e_2)).(pbase)) =s ("granules")));
+            rely ((((((ret_rtt.(e_2)).(poffset)) + (8)) mod (16)) = (8)));
+            when st_18 == (
+                (granule_unlock_spec
+                  (ret_rtt.(e_2))
+                  ((st_4.[share].[globals].[g_granules] :<
+                    ((((st_4.(share)).(globals)).(g_granules)) #
+                      ((((ret_rtt.(e_2)).(poffset)) + (8)) / (16)) ==
+                      (((((st_4.(share)).(globals)).(g_granules)) @ ((((ret_rtt.(e_2)).(poffset)) + (8)) / (16))).[e_ref] :<
+                        ((((((st_4.(share)).(globals)).(g_granules)) @ ((((ret_rtt.(e_2)).(poffset)) + (8)) / (16))).(e_ref)).[e_u_anon_3_0] :<
+                          (((((((st_4.(share)).(globals)).(g_granules)) @ ((((ret_rtt.(e_2)).(poffset)) + (8)) / (16))).(e_ref)).(e_u_anon_3_0)) + (1)))))).[share].[granule_data] :<
+                    (((st_4.(share)).(granule_data)) #
+                      ((((ret_rtt.(e_2)).(poffset)) + ((8 * ((ret_rtt.(e_3)))))) / (4096)) ==
+                      ((((st_4.(share)).(granule_data)) @ ((((ret_rtt.(e_2)).(poffset)) + ((8 * ((ret_rtt.(e_3)))))) / (4096))).[g_norm] :<
+                        (((((st_4.(share)).(granule_data)) @ ((((ret_rtt.(e_2)).(poffset)) + ((8 * ((ret_rtt.(e_3)))))) / (4096))).(g_norm)) #
+                          ((((ret_rtt.(e_2)).(poffset)) + ((8 * ((ret_rtt.(e_3)))))) mod (4096)) ==
+                          (test_PTE_Z (test_Z_PTE v_3))))))));
+            (Some (0, st_18)))
+          else (
+            when st_1 == ((spinlock_acquire_spec (mkPtr "granules" (((test_Z_PTE v_3).(meta_PA)).(meta_granule_offset))) st_4));
+            if ((((((st_1.(share)).(globals)).(g_granules)) @ ((((test_Z_PTE v_3).(meta_PA)).(meta_granule_offset)) / (16))).(e_state_s_granule)) =? (0))
             then (
-              when st_10 == (
-                  (s2tt_init_unassigned_spec
-                    (mkPtr "granule_data" ((test_PA v_1).(meta_granule_offset)))
-                    ((abs_tte_read (mkPtr "granule_data" (((ret_record.(e_2)).(poffset)) + ((8 * ((ret_record.(e_3))))))) st_4).(meta_ripas))
-                    st_4));
-              rely ((((((ret_record.(e_2)).(poffset)) + (8)) mod (16)) = (8)));
-              rely (((((test_PA v_1).(meta_granule_offset)) mod (16)) = (0)));
-              when st_16 == (
+              rely (((((((test_Z_PTE v_3).(meta_PA)).(meta_granule_offset)) mod (16)) = (0)) /\ (((((test_Z_PTE v_3).(meta_PA)).(meta_granule_offset)) >= (0)))));
+              when st_6 == (
                   (granule_unlock_spec
-                    (ret_record.(e_2))
-                    ((st_10.[share].[globals].[g_granules] :<
-                      (((((st_10.(share)).(globals)).(g_granules)) #
-                        ((((ret_record.(e_2)).(poffset)) + (8)) / (16)) ==
-                        (((((st_10.(share)).(globals)).(g_granules)) @ ((((ret_record.(e_2)).(poffset)) + (8)) / (16))).[e_ref] :<
-                          ((((((st_10.(share)).(globals)).(g_granules)) @ ((((ret_record.(e_2)).(poffset)) + (8)) / (16))).(e_ref)).[e_u_anon_3_0] :<
-                            (((((((st_10.(share)).(globals)).(g_granules)) @ ((((ret_record.(e_2)).(poffset)) + (8)) / (16))).(e_ref)).(e_u_anon_3_0)) + (1))))) #
-                        ((((test_PA v_1).(meta_granule_offset)) + (4)) / (16)) ==
-                        ((((((st_10.(share)).(globals)).(g_granules)) #
-                          ((((ret_record.(e_2)).(poffset)) + (8)) / (16)) ==
-                          (((((st_10.(share)).(globals)).(g_granules)) @ ((((ret_record.(e_2)).(poffset)) + (8)) / (16))).[e_ref] :<
-                            ((((((st_10.(share)).(globals)).(g_granules)) @ ((((ret_record.(e_2)).(poffset)) + (8)) / (16))).(e_ref)).[e_u_anon_3_0] :<
-                              (((((((st_10.(share)).(globals)).(g_granules)) @ ((((ret_record.(e_2)).(poffset)) + (8)) / (16))).(e_ref)).(e_u_anon_3_0)) + (1))))) @ ((((test_PA v_1).(meta_granule_offset)) + (4)) / (16))).[e_state_s_granule] :<
-                          5))).[share].[granule_data] :<
-                      (((st_10.(share)).(granule_data)) #
-                        ((((ret_record.(e_2)).(poffset)) + ((8 * ((ret_record.(e_3)))))) / (4096)) ==
-                        ((((st_10.(share)).(granule_data)) @ ((((ret_record.(e_2)).(poffset)) + ((8 * ((ret_record.(e_3)))))) / (4096))).[g_norm] :<
-                          (((((st_10.(share)).(granule_data)) @ ((((ret_record.(e_2)).(poffset)) + ((8 * ((ret_record.(e_3)))))) / (4096))).(g_norm)) #
-                            ((((ret_record.(e_2)).(poffset)) + ((8 * ((ret_record.(e_3)))))) mod (4096)) ==
-                            (test_PTE_Z (mkabs_PTE_t (test_PA v_1) 3 0))))))));
-              when st_17 == ((granule_unlock_spec (mkPtr "granules" ((test_PA v_1).(meta_granule_offset))) st_16));
-              (Some (0, st_17)))
+                    (mkPtr "granules" (((test_Z_PTE v_3).(meta_PA)).(meta_granule_offset)))
+                    (st_1.[share].[globals].[g_granules] :<
+                      ((((st_1.(share)).(globals)).(g_granules)) #
+                        ((((test_Z_PTE v_3).(meta_PA)).(meta_granule_offset)) / (16)) ==
+                        ((((((st_1.(share)).(globals)).(g_granules)) @ ((((test_Z_PTE v_3).(meta_PA)).(meta_granule_offset)) / (16))).[e_ref] :<
+                          ((((((st_1.(share)).(globals)).(g_granules)) @ ((((test_Z_PTE v_3).(meta_PA)).(meta_granule_offset)) / (16))).(e_ref)).[e_u_anon_3_0] :<
+                            ((g_mapped_addr_set_para
+                              ((((((st_1.(share)).(globals)).(g_granules)) @ ((((test_Z_PTE v_3).(meta_PA)).(meta_granule_offset)) / (16))).(e_ref)).(e_u_anon_3_0))
+                              v_1) +
+                              (1)))).[e_state_s_granule] :<
+                          6)))));
+              rely ((((ret_rtt.(e_2)).(pbase)) =s ("granules")));
+              rely ((((((ret_rtt.(e_2)).(poffset)) + (8)) mod (16)) = (8)));
+              when st_19 == (
+                  (granule_unlock_spec
+                    (ret_rtt.(e_2))
+                    ((st_6.[share].[globals].[g_granules] :<
+                      ((((st_6.(share)).(globals)).(g_granules)) #
+                        ((((ret_rtt.(e_2)).(poffset)) + (8)) / (16)) ==
+                        (((((st_6.(share)).(globals)).(g_granules)) @ ((((ret_rtt.(e_2)).(poffset)) + (8)) / (16))).[e_ref] :<
+                          ((((((st_6.(share)).(globals)).(g_granules)) @ ((((ret_rtt.(e_2)).(poffset)) + (8)) / (16))).(e_ref)).[e_u_anon_3_0] :<
+                            (((((((st_6.(share)).(globals)).(g_granules)) @ ((((ret_rtt.(e_2)).(poffset)) + (8)) / (16))).(e_ref)).(e_u_anon_3_0)) + (1)))))).[share].[granule_data] :<
+                      (((st_6.(share)).(granule_data)) #
+                        ((((ret_rtt.(e_2)).(poffset)) + ((8 * ((ret_rtt.(e_3)))))) / (4096)) ==
+                        ((((st_6.(share)).(granule_data)) @ ((((ret_rtt.(e_2)).(poffset)) + ((8 * ((ret_rtt.(e_3)))))) / (4096))).[g_norm] :<
+                          (((((st_6.(share)).(granule_data)) @ ((((ret_rtt.(e_2)).(poffset)) + ((8 * ((ret_rtt.(e_3)))))) / (4096))).(g_norm)) #
+                            ((((ret_rtt.(e_2)).(poffset)) + ((8 * ((ret_rtt.(e_3)))))) mod (4096)) ==
+                            (test_PTE_Z (test_Z_PTE v_3))))))));
+              (Some (0, st_19)))
             else (
-              if (((v_3 + ((- 1))) <? (3)) && ((((abs_tte_read (mkPtr "granule_data" (((ret_record.(e_2)).(poffset)) + ((8 * ((ret_record.(e_3))))))) st_4).(meta_desc_type)) =? (3))))
+              when st_2 == ((spinlock_release_spec (mkPtr "granules" (((test_Z_PTE v_3).(meta_PA)).(meta_granule_offset))) st_1));
+              when st_5 == ((spinlock_acquire_spec (mkPtr "granules" (((test_Z_PTE v_3).(meta_PA)).(meta_granule_offset))) st_2));
+              if (((((((st_5.(share)).(globals)).(g_granules)) @ ((((test_Z_PTE v_3).(meta_PA)).(meta_granule_offset)) / (16))).(e_state_s_granule)) - (6)) =? (0))
               then (
-                match (
-                  match (
-                    when st_11 == ((granule_unlock_spec (ret_record.(e_2)) st_4));
-                    when st_12 == ((granule_unlock_spec (mkPtr "granules" ((test_PA v_1).(meta_granule_offset))) st_11));
-                    (Some (true, (pack_struct_return_code_para (make_return_code_para 9)), st_12))
-                  ) with
-                  | (Some (return___1, retval___1, st_10)) => (Some (return___1, retval___1, st_10))
-                  | _ => None
-                  end
-                ) with
-                | (Some (return___1, retval___1, st_10)) =>
-                  if return___1
-                  then (Some (retval___1, st_10))
-                  else (
-                    rely (((((test_PA v_1).(meta_granule_offset)) mod (16)) = (0)));
-                    when st_14 == (
-                        (granule_unlock_spec
-                          (ret_record.(e_2))
-                          ((st_10.[share].[globals].[g_granules] :<
-                            ((((st_10.(share)).(globals)).(g_granules)) #
-                              ((((test_PA v_1).(meta_granule_offset)) + (4)) / (16)) ==
-                              (((((st_10.(share)).(globals)).(g_granules)) @ ((((test_PA v_1).(meta_granule_offset)) + (4)) / (16))).[e_state_s_granule] :< 5))).[share].[granule_data] :<
-                            (((st_10.(share)).(granule_data)) #
-                              ((((ret_record.(e_2)).(poffset)) + ((8 * ((ret_record.(e_3)))))) / (4096)) ==
-                              ((((st_10.(share)).(granule_data)) @ ((((ret_record.(e_2)).(poffset)) + ((8 * ((ret_record.(e_3)))))) / (4096))).[g_norm] :<
-                                (((((st_10.(share)).(granule_data)) @ ((((ret_record.(e_2)).(poffset)) + ((8 * ((ret_record.(e_3)))))) / (4096))).(g_norm)) #
-                                  ((((ret_record.(e_2)).(poffset)) + ((8 * ((ret_record.(e_3)))))) mod (4096)) ==
-                                  (test_PTE_Z (mkabs_PTE_t (test_PA v_1) 3 0))))))));
-                    when st_15 == ((granule_unlock_spec (mkPtr "granules" ((test_PA v_1).(meta_granule_offset))) st_14));
-                    (Some (0, st_15)))
-                | None => None
-                end)
-              else (
-                rely (((((test_PA v_1).(meta_granule_offset)) mod (16)) = (0)));
-                when st_14 == (
+                rely (((((((test_Z_PTE v_3).(meta_PA)).(meta_granule_offset)) mod (16)) = (0)) /\ (((((test_Z_PTE v_3).(meta_PA)).(meta_granule_offset)) >= (0)))));
+                rely (((((((test_Z_PTE v_3).(meta_PA)).(meta_granule_offset)) + (8)) mod (16)) = (8)));
+                when st_6 == (
                     (granule_unlock_spec
-                      (ret_record.(e_2))
+                      (mkPtr "granules" (((test_Z_PTE v_3).(meta_PA)).(meta_granule_offset)))
+                      (st_5.[share].[globals].[g_granules] :<
+                        ((((st_5.(share)).(globals)).(g_granules)) #
+                          ((((test_Z_PTE v_3).(meta_PA)).(meta_granule_offset)) / (16)) ==
+                          (((((st_5.(share)).(globals)).(g_granules)) @ ((((test_Z_PTE v_3).(meta_PA)).(meta_granule_offset)) / (16))).[e_ref] :<
+                            ((((((st_5.(share)).(globals)).(g_granules)) @ ((((test_Z_PTE v_3).(meta_PA)).(meta_granule_offset)) / (16))).(e_ref)).[e_u_anon_3_0] :<
+                              (((((((st_5.(share)).(globals)).(g_granules)) @ ((((test_Z_PTE v_3).(meta_PA)).(meta_granule_offset)) / (16))).(e_ref)).(e_u_anon_3_0)) + (1))))))));
+                rely ((true = (true)));
+                rely ((((ret_rtt.(e_2)).(pbase)) =s ("granules")));
+                rely ((((((ret_rtt.(e_2)).(poffset)) + (8)) mod (16)) = (8)));
+                when st_19 == (
+                    (granule_unlock_spec
+                      (ret_rtt.(e_2))
+                      ((st_6.[share].[globals].[g_granules] :<
+                        ((((st_6.(share)).(globals)).(g_granules)) #
+                          ((((ret_rtt.(e_2)).(poffset)) + (8)) / (16)) ==
+                          (((((st_6.(share)).(globals)).(g_granules)) @ ((((ret_rtt.(e_2)).(poffset)) + (8)) / (16))).[e_ref] :<
+                            ((((((st_6.(share)).(globals)).(g_granules)) @ ((((ret_rtt.(e_2)).(poffset)) + (8)) / (16))).(e_ref)).[e_u_anon_3_0] :<
+                              (((((((st_6.(share)).(globals)).(g_granules)) @ ((((ret_rtt.(e_2)).(poffset)) + (8)) / (16))).(e_ref)).(e_u_anon_3_0)) + (1)))))).[share].[granule_data] :<
+                        (((st_6.(share)).(granule_data)) #
+                          ((((ret_rtt.(e_2)).(poffset)) + ((8 * ((ret_rtt.(e_3)))))) / (4096)) ==
+                          ((((st_6.(share)).(granule_data)) @ ((((ret_rtt.(e_2)).(poffset)) + ((8 * ((ret_rtt.(e_3)))))) / (4096))).[g_norm] :<
+                            (((((st_6.(share)).(granule_data)) @ ((((ret_rtt.(e_2)).(poffset)) + ((8 * ((ret_rtt.(e_3)))))) / (4096))).(g_norm)) #
+                              ((((ret_rtt.(e_2)).(poffset)) + ((8 * ((ret_rtt.(e_3)))))) mod (4096)) ==
+                              (test_PTE_Z (test_Z_PTE v_3))))))));
+                (Some (0, st_19)))
+              else (
+                when st_6 == ((spinlock_release_spec (mkPtr "granules" (((test_Z_PTE v_3).(meta_PA)).(meta_granule_offset))) st_5));
+                if ((pack_struct_return_code_para (make_return_code_para 1)) =? (0))
+                then (
+                  rely ((((ret_rtt.(e_2)).(pbase)) =s ("granules")));
+                  rely ((((((ret_rtt.(e_2)).(poffset)) + (8)) mod (16)) = (8)));
+                  when st_19 == (
+                      (granule_unlock_spec
+                        (ret_rtt.(e_2))
+                        ((st_6.[share].[globals].[g_granules] :<
+                          ((((st_6.(share)).(globals)).(g_granules)) #
+                            ((((ret_rtt.(e_2)).(poffset)) + (8)) / (16)) ==
+                            (((((st_6.(share)).(globals)).(g_granules)) @ ((((ret_rtt.(e_2)).(poffset)) + (8)) / (16))).[e_ref] :<
+                              ((((((st_6.(share)).(globals)).(g_granules)) @ ((((ret_rtt.(e_2)).(poffset)) + (8)) / (16))).(e_ref)).[e_u_anon_3_0] :<
+                                (((((((st_6.(share)).(globals)).(g_granules)) @ ((((ret_rtt.(e_2)).(poffset)) + (8)) / (16))).(e_ref)).(e_u_anon_3_0)) + (1)))))).[share].[granule_data] :<
+                          (((st_6.(share)).(granule_data)) #
+                            ((((ret_rtt.(e_2)).(poffset)) + ((8 * ((ret_rtt.(e_3)))))) / (4096)) ==
+                            ((((st_6.(share)).(granule_data)) @ ((((ret_rtt.(e_2)).(poffset)) + ((8 * ((ret_rtt.(e_3)))))) / (4096))).[g_norm] :<
+                              (((((st_6.(share)).(granule_data)) @ ((((ret_rtt.(e_2)).(poffset)) + ((8 * ((ret_rtt.(e_3)))))) / (4096))).(g_norm)) #
+                                ((((ret_rtt.(e_2)).(poffset)) + ((8 * ((ret_rtt.(e_3)))))) mod (4096)) ==
+                                (test_PTE_Z (test_Z_PTE v_3))))))));
+                  (Some (0, st_19)))
+                else (
+                  when st_14 == ((granule_unlock_spec (ret_rtt.(e_2)) st_6));
+                  (Some ((pack_struct_return_code_para (make_return_code_para 1)), st_14)))))))
+        else (
+          when st_13 == ((granule_unlock_spec (ret_rtt.(e_2)) st_4));
+          (Some ((pack_struct_return_code_para (make_return_code_para 9)), st_13))))
+      else (
+        if (v_4 =? (1))
+        then (
+          if ((v_2 =? (3)) && ((((abs_tte_read (mkPtr "granule_data" (((ret_rtt.(e_2)).(poffset)) + ((8 * ((ret_rtt.(e_3))))))) st_4).(meta_desc_type)) =? (3))))
+          then (
+            if (uart0_phys_para (abs_tte_read (mkPtr "granule_data" (((ret_rtt.(e_2)).(poffset)) + ((8 * ((ret_rtt.(e_3))))))) st_4))
+            then (
+              rely ((((((ret_rtt.(e_2)).(pbase)) = ("granules")) /\ (((((ret_rtt.(e_2)).(poffset)) mod (16)) = (0)))) /\ ((((ret_rtt.(e_2)).(poffset)) >= (0)))));
+              when st_19 == (
+                  (granule_unlock_spec
+                    (ret_rtt.(e_2))
+                    ((st_4.[share].[globals].[g_granules] :<
+                      ((((st_4.(share)).(globals)).(g_granules)) #
+                        (((ret_rtt.(e_2)).(poffset)) / (16)) ==
+                        (((((st_4.(share)).(globals)).(g_granules)) @ (((ret_rtt.(e_2)).(poffset)) / (16))).[e_ref] :<
+                          ((((((st_4.(share)).(globals)).(g_granules)) @ (((ret_rtt.(e_2)).(poffset)) / (16))).(e_ref)).[e_u_anon_3_0] :<
+                            (((((((st_4.(share)).(globals)).(g_granules)) @ (((ret_rtt.(e_2)).(poffset)) / (16))).(e_ref)).(e_u_anon_3_0)) + ((- 1))))))).[share].[granule_data] :<
+                      (((st_4.(share)).(granule_data)) #
+                        ((((ret_rtt.(e_2)).(poffset)) + ((8 * ((ret_rtt.(e_3)))))) / (4096)) ==
+                        ((((st_4.(share)).(granule_data)) @ ((((ret_rtt.(e_2)).(poffset)) + ((8 * ((ret_rtt.(e_3)))))) / (4096))).[g_norm] :<
+                          (((((st_4.(share)).(granule_data)) @ ((((ret_rtt.(e_2)).(poffset)) + ((8 * ((ret_rtt.(e_3)))))) / (4096))).(g_norm)) #
+                            ((((ret_rtt.(e_2)).(poffset)) + ((8 * ((ret_rtt.(e_3)))))) mod (4096)) ==
+                            (test_PTE_Z (mkabs_PTE_t (mkabs_PA_t (- 1)) 0 1))))))));
+              (Some (0, st_19)))
+            else (
+              when st_1 == (
+                  (spinlock_acquire_spec
+                    (mkPtr "granules" (((abs_tte_read (mkPtr "granule_data" (((ret_rtt.(e_2)).(poffset)) + ((8 * ((ret_rtt.(e_3))))))) st_4).(meta_PA)).(meta_granule_offset)))
+                    st_4));
+              if (
+                (((((((st_1.(share)).(globals)).(g_granules)) @ ((((abs_tte_read (mkPtr "granule_data" (((ret_rtt.(e_2)).(poffset)) + ((8 * ((ret_rtt.(e_3))))))) st_4).(meta_PA)).(meta_granule_offset)) / (16))).(e_state_s_granule)) -
+                  (6)) =?
+                  (0)))
+              then (
+                rely (
+                  ((((((abs_tte_read (mkPtr "granule_data" (((ret_rtt.(e_2)).(poffset)) + ((8 * ((ret_rtt.(e_3))))))) st_4).(meta_PA)).(meta_granule_offset)) mod (16)) = (0)) /\
+                    (((((abs_tte_read (mkPtr "granule_data" (((ret_rtt.(e_2)).(poffset)) + ((8 * ((ret_rtt.(e_3))))))) st_4).(meta_PA)).(meta_granule_offset)) >= (0)))));
+                if (
+                  ((g_refcount_para
+                    (mkPtr "granules" (((abs_tte_read (mkPtr "granule_data" (((ret_rtt.(e_2)).(poffset)) + ((8 * ((ret_rtt.(e_3))))))) st_4).(meta_PA)).(meta_granule_offset)))
+                    (st_1.[share].[globals].[g_granules] :<
+                      ((((st_1.(share)).(globals)).(g_granules)) #
+                        ((((abs_tte_read (mkPtr "granule_data" (((ret_rtt.(e_2)).(poffset)) + ((8 * ((ret_rtt.(e_3))))))) st_4).(meta_PA)).(meta_granule_offset)) / (16)) ==
+                        (((((st_1.(share)).(globals)).(g_granules)) @ ((((abs_tte_read (mkPtr "granule_data" (((ret_rtt.(e_2)).(poffset)) + ((8 * ((ret_rtt.(e_3))))))) st_4).(meta_PA)).(meta_granule_offset)) / (16))).[e_ref] :<
+                          ((((((st_1.(share)).(globals)).(g_granules)) @ ((((abs_tte_read (mkPtr "granule_data" (((ret_rtt.(e_2)).(poffset)) + ((8 * ((ret_rtt.(e_3))))))) st_4).(meta_PA)).(meta_granule_offset)) / (16))).(e_ref)).[e_u_anon_3_0] :<
+                            (((((((st_1.(share)).(globals)).(g_granules)) @ ((((abs_tte_read (mkPtr "granule_data" (((ret_rtt.(e_2)).(poffset)) + ((8 * ((ret_rtt.(e_3))))))) st_4).(meta_PA)).(meta_granule_offset)) / (16))).(e_ref)).(e_u_anon_3_0)) +
+                              ((- 1)))))))) =?
+                    (0)))
+                then (
+                  when st_7 == (
+                      (granule_unlock_spec
+                        (mkPtr "granules" (((abs_tte_read (mkPtr "granule_data" (((ret_rtt.(e_2)).(poffset)) + ((8 * ((ret_rtt.(e_3))))))) st_4).(meta_PA)).(meta_granule_offset)))
+                        (st_1.[share].[globals].[g_granules] :<
+                          ((((st_1.(share)).(globals)).(g_granules)) #
+                            ((((abs_tte_read (mkPtr "granule_data" (((ret_rtt.(e_2)).(poffset)) + ((8 * ((ret_rtt.(e_3))))))) st_4).(meta_PA)).(meta_granule_offset)) / (16)) ==
+                            ((((((st_1.(share)).(globals)).(g_granules)) @ ((((abs_tte_read (mkPtr "granule_data" (((ret_rtt.(e_2)).(poffset)) + ((8 * ((ret_rtt.(e_3))))))) st_4).(meta_PA)).(meta_granule_offset)) / (16))).[e_ref] :<
+                              ((((((st_1.(share)).(globals)).(g_granules)) @ ((((abs_tte_read (mkPtr "granule_data" (((ret_rtt.(e_2)).(poffset)) + ((8 * ((ret_rtt.(e_3))))))) st_4).(meta_PA)).(meta_granule_offset)) / (16))).(e_ref)).[e_u_anon_3_0] :<
+                                (g_mapped_addr_set_para
+                                  (((((((st_1.(share)).(globals)).(g_granules)) @ ((((abs_tte_read (mkPtr "granule_data" (((ret_rtt.(e_2)).(poffset)) + ((8 * ((ret_rtt.(e_3))))))) st_4).(meta_PA)).(meta_granule_offset)) / (16))).(e_ref)).(e_u_anon_3_0)) +
+                                    ((- 1)))
+                                  0))).[e_state_s_granule] :<
+                              0)))));
+                  rely ((((((ret_rtt.(e_2)).(pbase)) = ("granules")) /\ (((((ret_rtt.(e_2)).(poffset)) mod (16)) = (0)))) /\ ((((ret_rtt.(e_2)).(poffset)) >= (0)))));
+                  when st_20 == (
+                      (granule_unlock_spec
+                        (ret_rtt.(e_2))
+                        ((st_7.[share].[globals].[g_granules] :<
+                          ((((st_7.(share)).(globals)).(g_granules)) #
+                            (((ret_rtt.(e_2)).(poffset)) / (16)) ==
+                            (((((st_7.(share)).(globals)).(g_granules)) @ (((ret_rtt.(e_2)).(poffset)) / (16))).[e_ref] :<
+                              ((((((st_7.(share)).(globals)).(g_granules)) @ (((ret_rtt.(e_2)).(poffset)) / (16))).(e_ref)).[e_u_anon_3_0] :<
+                                (((((((st_7.(share)).(globals)).(g_granules)) @ (((ret_rtt.(e_2)).(poffset)) / (16))).(e_ref)).(e_u_anon_3_0)) + ((- 1))))))).[share].[granule_data] :<
+                          (((st_7.(share)).(granule_data)) #
+                            ((((ret_rtt.(e_2)).(poffset)) + ((8 * ((ret_rtt.(e_3)))))) / (4096)) ==
+                            ((((st_7.(share)).(granule_data)) @ ((((ret_rtt.(e_2)).(poffset)) + ((8 * ((ret_rtt.(e_3)))))) / (4096))).[g_norm] :<
+                              (((((st_7.(share)).(granule_data)) @ ((((ret_rtt.(e_2)).(poffset)) + ((8 * ((ret_rtt.(e_3)))))) / (4096))).(g_norm)) #
+                                ((((ret_rtt.(e_2)).(poffset)) + ((8 * ((ret_rtt.(e_3)))))) mod (4096)) ==
+                                (test_PTE_Z (mkabs_PTE_t (mkabs_PA_t (- 1)) 0 1))))))));
+                  (Some (0, st_20)))
+                else (
+                  when st_5 == (
+                      (granule_unlock_spec
+                        (mkPtr "granules" (((abs_tte_read (mkPtr "granule_data" (((ret_rtt.(e_2)).(poffset)) + ((8 * ((ret_rtt.(e_3))))))) st_4).(meta_PA)).(meta_granule_offset)))
+                        (st_1.[share].[globals].[g_granules] :<
+                          ((((st_1.(share)).(globals)).(g_granules)) #
+                            ((((abs_tte_read (mkPtr "granule_data" (((ret_rtt.(e_2)).(poffset)) + ((8 * ((ret_rtt.(e_3))))))) st_4).(meta_PA)).(meta_granule_offset)) / (16)) ==
+                            (((((st_1.(share)).(globals)).(g_granules)) @ ((((abs_tte_read (mkPtr "granule_data" (((ret_rtt.(e_2)).(poffset)) + ((8 * ((ret_rtt.(e_3))))))) st_4).(meta_PA)).(meta_granule_offset)) / (16))).[e_ref] :<
+                              ((((((st_1.(share)).(globals)).(g_granules)) @ ((((abs_tte_read (mkPtr "granule_data" (((ret_rtt.(e_2)).(poffset)) + ((8 * ((ret_rtt.(e_3))))))) st_4).(meta_PA)).(meta_granule_offset)) / (16))).(e_ref)).[e_u_anon_3_0] :<
+                                (g_mapped_addr_set_para
+                                  (((((((st_1.(share)).(globals)).(g_granules)) @ ((((abs_tte_read (mkPtr "granule_data" (((ret_rtt.(e_2)).(poffset)) + ((8 * ((ret_rtt.(e_3))))))) st_4).(meta_PA)).(meta_granule_offset)) / (16))).(e_ref)).(e_u_anon_3_0)) +
+                                    ((- 1)))
+                                  0)))))));
+                  rely ((((((ret_rtt.(e_2)).(pbase)) = ("granules")) /\ (((((ret_rtt.(e_2)).(poffset)) mod (16)) = (0)))) /\ ((((ret_rtt.(e_2)).(poffset)) >= (0)))));
+                  when st_20 == (
+                      (granule_unlock_spec
+                        (ret_rtt.(e_2))
+                        ((st_5.[share].[globals].[g_granules] :<
+                          ((((st_5.(share)).(globals)).(g_granules)) #
+                            (((ret_rtt.(e_2)).(poffset)) / (16)) ==
+                            (((((st_5.(share)).(globals)).(g_granules)) @ (((ret_rtt.(e_2)).(poffset)) / (16))).[e_ref] :<
+                              ((((((st_5.(share)).(globals)).(g_granules)) @ (((ret_rtt.(e_2)).(poffset)) / (16))).(e_ref)).[e_u_anon_3_0] :<
+                                (((((((st_5.(share)).(globals)).(g_granules)) @ (((ret_rtt.(e_2)).(poffset)) / (16))).(e_ref)).(e_u_anon_3_0)) + ((- 1))))))).[share].[granule_data] :<
+                          (((st_5.(share)).(granule_data)) #
+                            ((((ret_rtt.(e_2)).(poffset)) + ((8 * ((ret_rtt.(e_3)))))) / (4096)) ==
+                            ((((st_5.(share)).(granule_data)) @ ((((ret_rtt.(e_2)).(poffset)) + ((8 * ((ret_rtt.(e_3)))))) / (4096))).[g_norm] :<
+                              (((((st_5.(share)).(granule_data)) @ ((((ret_rtt.(e_2)).(poffset)) + ((8 * ((ret_rtt.(e_3)))))) / (4096))).(g_norm)) #
+                                ((((ret_rtt.(e_2)).(poffset)) + ((8 * ((ret_rtt.(e_3)))))) mod (4096)) ==
+                                (test_PTE_Z (mkabs_PTE_t (mkabs_PA_t (- 1)) 0 1))))))));
+                  (Some (0, st_20))))
+              else (
+                when st_2 == (
+                    (spinlock_release_spec
+                      (mkPtr "granules" (((abs_tte_read (mkPtr "granule_data" (((ret_rtt.(e_2)).(poffset)) + ((8 * ((ret_rtt.(e_3))))))) st_4).(meta_PA)).(meta_granule_offset)))
+                      st_1));
+                if ((pack_struct_return_code_para (make_return_code_para 1)) =? (0))
+                then (
+                  rely ((((((ret_rtt.(e_2)).(pbase)) = ("granules")) /\ (((((ret_rtt.(e_2)).(poffset)) mod (16)) = (0)))) /\ ((((ret_rtt.(e_2)).(poffset)) >= (0)))));
+                  when st_20 == (
+                      (granule_unlock_spec
+                        (ret_rtt.(e_2))
+                        ((st_2.[share].[globals].[g_granules] :<
+                          ((((st_2.(share)).(globals)).(g_granules)) #
+                            (((ret_rtt.(e_2)).(poffset)) / (16)) ==
+                            (((((st_2.(share)).(globals)).(g_granules)) @ (((ret_rtt.(e_2)).(poffset)) / (16))).[e_ref] :<
+                              ((((((st_2.(share)).(globals)).(g_granules)) @ (((ret_rtt.(e_2)).(poffset)) / (16))).(e_ref)).[e_u_anon_3_0] :<
+                                (((((((st_2.(share)).(globals)).(g_granules)) @ (((ret_rtt.(e_2)).(poffset)) / (16))).(e_ref)).(e_u_anon_3_0)) + ((- 1))))))).[share].[granule_data] :<
+                          (((st_2.(share)).(granule_data)) #
+                            ((((ret_rtt.(e_2)).(poffset)) + ((8 * ((ret_rtt.(e_3)))))) / (4096)) ==
+                            ((((st_2.(share)).(granule_data)) @ ((((ret_rtt.(e_2)).(poffset)) + ((8 * ((ret_rtt.(e_3)))))) / (4096))).[g_norm] :<
+                              (((((st_2.(share)).(granule_data)) @ ((((ret_rtt.(e_2)).(poffset)) + ((8 * ((ret_rtt.(e_3)))))) / (4096))).(g_norm)) #
+                                ((((ret_rtt.(e_2)).(poffset)) + ((8 * ((ret_rtt.(e_3)))))) mod (4096)) ==
+                                (test_PTE_Z (mkabs_PTE_t (mkabs_PA_t (- 1)) 0 1))))))));
+                  (Some (0, st_20)))
+                else (
+                  when st_14 == ((granule_unlock_spec (ret_rtt.(e_2)) st_2));
+                  (Some ((pack_struct_return_code_para (make_return_code_para 1)), st_14))))))
+          else (
+            if ((v_2 <>? (3)) && ((((abs_tte_read (mkPtr "granule_data" (((ret_rtt.(e_2)).(poffset)) + ((8 * ((ret_rtt.(e_3))))))) st_4).(meta_desc_type)) =? (1))))
+            then (
+              if (uart0_phys_para (abs_tte_read (mkPtr "granule_data" (((ret_rtt.(e_2)).(poffset)) + ((8 * ((ret_rtt.(e_3))))))) st_4))
+              then (
+                rely ((((((ret_rtt.(e_2)).(pbase)) = ("granules")) /\ (((((ret_rtt.(e_2)).(poffset)) mod (16)) = (0)))) /\ ((((ret_rtt.(e_2)).(poffset)) >= (0)))));
+                when st_19 == (
+                    (granule_unlock_spec
+                      (ret_rtt.(e_2))
                       ((st_4.[share].[globals].[g_granules] :<
                         ((((st_4.(share)).(globals)).(g_granules)) #
-                          ((((test_PA v_1).(meta_granule_offset)) + (4)) / (16)) ==
-                          (((((st_4.(share)).(globals)).(g_granules)) @ ((((test_PA v_1).(meta_granule_offset)) + (4)) / (16))).[e_state_s_granule] :< 5))).[share].[granule_data] :<
+                          (((ret_rtt.(e_2)).(poffset)) / (16)) ==
+                          (((((st_4.(share)).(globals)).(g_granules)) @ (((ret_rtt.(e_2)).(poffset)) / (16))).[e_ref] :<
+                            ((((((st_4.(share)).(globals)).(g_granules)) @ (((ret_rtt.(e_2)).(poffset)) / (16))).(e_ref)).[e_u_anon_3_0] :<
+                              (((((((st_4.(share)).(globals)).(g_granules)) @ (((ret_rtt.(e_2)).(poffset)) / (16))).(e_ref)).(e_u_anon_3_0)) + ((- 1))))))).[share].[granule_data] :<
                         (((st_4.(share)).(granule_data)) #
-                          ((((ret_record.(e_2)).(poffset)) + ((8 * ((ret_record.(e_3)))))) / (4096)) ==
-                          ((((st_4.(share)).(granule_data)) @ ((((ret_record.(e_2)).(poffset)) + ((8 * ((ret_record.(e_3)))))) / (4096))).[g_norm] :<
-                            (((((st_4.(share)).(granule_data)) @ ((((ret_record.(e_2)).(poffset)) + ((8 * ((ret_record.(e_3)))))) / (4096))).(g_norm)) #
-                              ((((ret_record.(e_2)).(poffset)) + ((8 * ((ret_record.(e_3)))))) mod (4096)) ==
-                              (test_PTE_Z (mkabs_PTE_t (test_PA v_1) 3 0))))))));
-                when st_15 == ((granule_unlock_spec (mkPtr "granules" ((test_PA v_1).(meta_granule_offset))) st_14));
-                (Some (0, st_15)))))
-          else (
-            if (((ret_record.(e_1)) - (v_3)) =? (0))
-            then (
-              match (
-                match (
-                  match (
-                    when st_6 == ((granule_unlock_spec (ret_record.(e_2)) st_4));
-                    when st_7 == ((granule_unlock_spec (mkPtr "granules" ((test_PA v_1).(meta_granule_offset))) st_6));
-                    (Some (true, (pack_struct_return_code_para (make_return_code_para 9)), st_7))
-                  ) with
-                  | (Some (__return___0, __retval___0, st_5)) => (Some (__return___0, __retval___0, st_5))
-                  | _ => None
-                  end
-                ) with
-                | (Some (__return___0, __retval___0, st_5)) =>
-                  if __return___0
-                  then (Some (true, __retval___0, st_5))
-                  else (
-                    when st_7 == ((granule_unlock_spec (ret_record.(e_2)) st_5));
-                    when st_8 == ((granule_unlock_spec (mkPtr "granules" ((test_PA v_1).(meta_granule_offset))) st_7));
-                    (Some (true, (pack_struct_return_code_para (make_return_code_para 8)), st_8)))
-                | _ => None
-                end
-              ) with
-              | (Some (__return___0, __retval___0, st_5)) =>
-                if __return___0
-                then (Some (__retval___0, st_5))
-                else (
+                          ((((ret_rtt.(e_2)).(poffset)) + ((8 * ((ret_rtt.(e_3)))))) / (4096)) ==
+                          ((((st_4.(share)).(granule_data)) @ ((((ret_rtt.(e_2)).(poffset)) + ((8 * ((ret_rtt.(e_3)))))) / (4096))).[g_norm] :<
+                            (((((st_4.(share)).(granule_data)) @ ((((ret_rtt.(e_2)).(poffset)) + ((8 * ((ret_rtt.(e_3)))))) / (4096))).(g_norm)) #
+                              ((((ret_rtt.(e_2)).(poffset)) + ((8 * ((ret_rtt.(e_3)))))) mod (4096)) ==
+                              (test_PTE_Z (mkabs_PTE_t (mkabs_PA_t (- 1)) 0 1))))))));
+                (Some (0, st_19)))
+              else (
+                when st_1 == (
+                    (spinlock_acquire_spec
+                      (mkPtr "granules" (((abs_tte_read (mkPtr "granule_data" (((ret_rtt.(e_2)).(poffset)) + ((8 * ((ret_rtt.(e_3))))))) st_4).(meta_PA)).(meta_granule_offset)))
+                      st_4));
+                if (
+                  (((((((st_1.(share)).(globals)).(g_granules)) @ ((((abs_tte_read (mkPtr "granule_data" (((ret_rtt.(e_2)).(poffset)) + ((8 * ((ret_rtt.(e_3))))))) st_4).(meta_PA)).(meta_granule_offset)) / (16))).(e_state_s_granule)) -
+                    (6)) =?
+                    (0)))
+                then (
+                  rely (
+                    ((((((abs_tte_read (mkPtr "granule_data" (((ret_rtt.(e_2)).(poffset)) + ((8 * ((ret_rtt.(e_3))))))) st_4).(meta_PA)).(meta_granule_offset)) mod (16)) = (0)) /\
+                      (((((abs_tte_read (mkPtr "granule_data" (((ret_rtt.(e_2)).(poffset)) + ((8 * ((ret_rtt.(e_3))))))) st_4).(meta_PA)).(meta_granule_offset)) >= (0)))));
                   if (
-                    ((((abs_tte_read (mkPtr "granule_data" (((ret_record.(e_2)).(poffset)) + ((8 * ((ret_record.(e_3))))))) st_5).(meta_desc_type)) =? (0)) &&
-                      ((((abs_tte_read (mkPtr "granule_data" (((ret_record.(e_2)).(poffset)) + ((8 * ((ret_record.(e_3))))))) st_5).(meta_ripas)) =? (0)))))
+                    ((g_refcount_para
+                      (mkPtr "granules" (((abs_tte_read (mkPtr "granule_data" (((ret_rtt.(e_2)).(poffset)) + ((8 * ((ret_rtt.(e_3))))))) st_4).(meta_PA)).(meta_granule_offset)))
+                      (st_1.[share].[globals].[g_granules] :<
+                        ((((st_1.(share)).(globals)).(g_granules)) #
+                          ((((abs_tte_read (mkPtr "granule_data" (((ret_rtt.(e_2)).(poffset)) + ((8 * ((ret_rtt.(e_3))))))) st_4).(meta_PA)).(meta_granule_offset)) / (16)) ==
+                          (((((st_1.(share)).(globals)).(g_granules)) @ ((((abs_tte_read (mkPtr "granule_data" (((ret_rtt.(e_2)).(poffset)) + ((8 * ((ret_rtt.(e_3))))))) st_4).(meta_PA)).(meta_granule_offset)) / (16))).[e_ref] :<
+                            ((((((st_1.(share)).(globals)).(g_granules)) @ ((((abs_tte_read (mkPtr "granule_data" (((ret_rtt.(e_2)).(poffset)) + ((8 * ((ret_rtt.(e_3))))))) st_4).(meta_PA)).(meta_granule_offset)) / (16))).(e_ref)).[e_u_anon_3_0] :<
+                              (((((((st_1.(share)).(globals)).(g_granules)) @ ((((abs_tte_read (mkPtr "granule_data" (((ret_rtt.(e_2)).(poffset)) + ((8 * ((ret_rtt.(e_3))))))) st_4).(meta_PA)).(meta_granule_offset)) / (16))).(e_ref)).(e_u_anon_3_0)) +
+                                ((- 1)))))))) =?
+                      (0)))
                   then (
-                    when st_11 == (
-                        (s2tt_init_unassigned_spec
-                          (mkPtr "granule_data" ((test_PA v_1).(meta_granule_offset)))
-                          ((abs_tte_read (mkPtr "granule_data" (((ret_record.(e_2)).(poffset)) + ((8 * ((ret_record.(e_3))))))) st_5).(meta_ripas))
-                          st_5));
-                    rely ((((((ret_record.(e_2)).(poffset)) + (8)) mod (16)) = (8)));
-                    rely (((((test_PA v_1).(meta_granule_offset)) mod (16)) = (0)));
-                    when st_17 == (
+                    when st_7 == (
                         (granule_unlock_spec
-                          (ret_record.(e_2))
-                          ((st_11.[share].[globals].[g_granules] :<
-                            (((((st_11.(share)).(globals)).(g_granules)) #
-                              ((((ret_record.(e_2)).(poffset)) + (8)) / (16)) ==
-                              (((((st_11.(share)).(globals)).(g_granules)) @ ((((ret_record.(e_2)).(poffset)) + (8)) / (16))).[e_ref] :<
-                                ((((((st_11.(share)).(globals)).(g_granules)) @ ((((ret_record.(e_2)).(poffset)) + (8)) / (16))).(e_ref)).[e_u_anon_3_0] :<
-                                  (((((((st_11.(share)).(globals)).(g_granules)) @ ((((ret_record.(e_2)).(poffset)) + (8)) / (16))).(e_ref)).(e_u_anon_3_0)) + (1))))) #
-                              ((((test_PA v_1).(meta_granule_offset)) + (4)) / (16)) ==
-                              ((((((st_11.(share)).(globals)).(g_granules)) #
-                                ((((ret_record.(e_2)).(poffset)) + (8)) / (16)) ==
-                                (((((st_11.(share)).(globals)).(g_granules)) @ ((((ret_record.(e_2)).(poffset)) + (8)) / (16))).[e_ref] :<
-                                  ((((((st_11.(share)).(globals)).(g_granules)) @ ((((ret_record.(e_2)).(poffset)) + (8)) / (16))).(e_ref)).[e_u_anon_3_0] :<
-                                    (((((((st_11.(share)).(globals)).(g_granules)) @ ((((ret_record.(e_2)).(poffset)) + (8)) / (16))).(e_ref)).(e_u_anon_3_0)) + (1))))) @ ((((test_PA v_1).(meta_granule_offset)) + (4)) / (16))).[e_state_s_granule] :<
-                                5))).[share].[granule_data] :<
-                            (((st_11.(share)).(granule_data)) #
-                              ((((ret_record.(e_2)).(poffset)) + ((8 * ((ret_record.(e_3)))))) / (4096)) ==
-                              ((((st_11.(share)).(granule_data)) @ ((((ret_record.(e_2)).(poffset)) + ((8 * ((ret_record.(e_3)))))) / (4096))).[g_norm] :<
-                                (((((st_11.(share)).(granule_data)) @ ((((ret_record.(e_2)).(poffset)) + ((8 * ((ret_record.(e_3)))))) / (4096))).(g_norm)) #
-                                  ((((ret_record.(e_2)).(poffset)) + ((8 * ((ret_record.(e_3)))))) mod (4096)) ==
-                                  (test_PTE_Z (mkabs_PTE_t (test_PA v_1) 3 0))))))));
-                    when st_18 == ((granule_unlock_spec (mkPtr "granules" ((test_PA v_1).(meta_granule_offset))) st_17));
-                    (Some (0, st_18)))
+                          (mkPtr "granules" (((abs_tte_read (mkPtr "granule_data" (((ret_rtt.(e_2)).(poffset)) + ((8 * ((ret_rtt.(e_3))))))) st_4).(meta_PA)).(meta_granule_offset)))
+                          (st_1.[share].[globals].[g_granules] :<
+                            ((((st_1.(share)).(globals)).(g_granules)) #
+                              ((((abs_tte_read (mkPtr "granule_data" (((ret_rtt.(e_2)).(poffset)) + ((8 * ((ret_rtt.(e_3))))))) st_4).(meta_PA)).(meta_granule_offset)) / (16)) ==
+                              ((((((st_1.(share)).(globals)).(g_granules)) @ ((((abs_tte_read (mkPtr "granule_data" (((ret_rtt.(e_2)).(poffset)) + ((8 * ((ret_rtt.(e_3))))))) st_4).(meta_PA)).(meta_granule_offset)) / (16))).[e_ref] :<
+                                ((((((st_1.(share)).(globals)).(g_granules)) @ ((((abs_tte_read (mkPtr "granule_data" (((ret_rtt.(e_2)).(poffset)) + ((8 * ((ret_rtt.(e_3))))))) st_4).(meta_PA)).(meta_granule_offset)) / (16))).(e_ref)).[e_u_anon_3_0] :<
+                                  (g_mapped_addr_set_para
+                                    (((((((st_1.(share)).(globals)).(g_granules)) @ ((((abs_tte_read (mkPtr "granule_data" (((ret_rtt.(e_2)).(poffset)) + ((8 * ((ret_rtt.(e_3))))))) st_4).(meta_PA)).(meta_granule_offset)) / (16))).(e_ref)).(e_u_anon_3_0)) +
+                                      ((- 1)))
+                                    0))).[e_state_s_granule] :<
+                                0)))));
+                    rely ((true = (true)));
+                    rely ((((((ret_rtt.(e_2)).(pbase)) = ("granules")) /\ (((((ret_rtt.(e_2)).(poffset)) mod (16)) = (0)))) /\ ((((ret_rtt.(e_2)).(poffset)) >= (0)))));
+                    when st_20 == (
+                        (granule_unlock_spec
+                          (ret_rtt.(e_2))
+                          ((st_7.[share].[globals].[g_granules] :<
+                            ((((st_7.(share)).(globals)).(g_granules)) #
+                              (((ret_rtt.(e_2)).(poffset)) / (16)) ==
+                              (((((st_7.(share)).(globals)).(g_granules)) @ (((ret_rtt.(e_2)).(poffset)) / (16))).[e_ref] :<
+                                ((((((st_7.(share)).(globals)).(g_granules)) @ (((ret_rtt.(e_2)).(poffset)) / (16))).(e_ref)).[e_u_anon_3_0] :<
+                                  (((((((st_7.(share)).(globals)).(g_granules)) @ (((ret_rtt.(e_2)).(poffset)) / (16))).(e_ref)).(e_u_anon_3_0)) + ((- 1))))))).[share].[granule_data] :<
+                            (((st_7.(share)).(granule_data)) #
+                              ((((ret_rtt.(e_2)).(poffset)) + ((8 * ((ret_rtt.(e_3)))))) / (4096)) ==
+                              ((((st_7.(share)).(granule_data)) @ ((((ret_rtt.(e_2)).(poffset)) + ((8 * ((ret_rtt.(e_3)))))) / (4096))).[g_norm] :<
+                                (((((st_7.(share)).(granule_data)) @ ((((ret_rtt.(e_2)).(poffset)) + ((8 * ((ret_rtt.(e_3)))))) / (4096))).(g_norm)) #
+                                  ((((ret_rtt.(e_2)).(poffset)) + ((8 * ((ret_rtt.(e_3)))))) mod (4096)) ==
+                                  (test_PTE_Z (mkabs_PTE_t (mkabs_PA_t (- 1)) 0 1))))))));
+                    (Some (0, st_20)))
                   else (
-                    if (((abs_tte_read (mkPtr "granule_data" (((ret_record.(e_2)).(poffset)) + ((8 * ((ret_record.(e_3))))))) st_5).(meta_desc_type)) =? (3))
-                    then (
-                      match (
-                        match (
-                          when st_12 == ((granule_unlock_spec (ret_record.(e_2)) st_5));
-                          when st_13 == ((granule_unlock_spec (mkPtr "granules" ((test_PA v_1).(meta_granule_offset))) st_12));
-                          (Some (true, (pack_struct_return_code_para (make_return_code_para 9)), st_13))
-                        ) with
-                        | (Some (return___1, retval___1, st_11)) => (Some (return___1, retval___1, st_11))
-                        | _ => None
-                        end
-                      ) with
-                      | (Some (return___1, retval___1, st_11)) =>
-                        if return___1
-                        then (Some (retval___1, st_11))
-                        else (
-                          rely (((((test_PA v_1).(meta_granule_offset)) mod (16)) = (0)));
-                          when st_15 == (
-                              (granule_unlock_spec
-                                (ret_record.(e_2))
-                                ((st_11.[share].[globals].[g_granules] :<
-                                  ((((st_11.(share)).(globals)).(g_granules)) #
-                                    ((((test_PA v_1).(meta_granule_offset)) + (4)) / (16)) ==
-                                    (((((st_11.(share)).(globals)).(g_granules)) @ ((((test_PA v_1).(meta_granule_offset)) + (4)) / (16))).[e_state_s_granule] :< 5))).[share].[granule_data] :<
-                                  (((st_11.(share)).(granule_data)) #
-                                    ((((ret_record.(e_2)).(poffset)) + ((8 * ((ret_record.(e_3)))))) / (4096)) ==
-                                    ((((st_11.(share)).(granule_data)) @ ((((ret_record.(e_2)).(poffset)) + ((8 * ((ret_record.(e_3)))))) / (4096))).[g_norm] :<
-                                      (((((st_11.(share)).(granule_data)) @ ((((ret_record.(e_2)).(poffset)) + ((8 * ((ret_record.(e_3)))))) / (4096))).(g_norm)) #
-                                        ((((ret_record.(e_2)).(poffset)) + ((8 * ((ret_record.(e_3)))))) mod (4096)) ==
-                                        (test_PTE_Z (mkabs_PTE_t (test_PA v_1) 3 0))))))));
-                          when st_16 == ((granule_unlock_spec (mkPtr "granules" ((test_PA v_1).(meta_granule_offset))) st_15));
-                          (Some (0, st_16)))
-                      | None => None
-                      end)
-                    else (
-                      rely (((((test_PA v_1).(meta_granule_offset)) mod (16)) = (0)));
-                      when st_15 == (
-                          (granule_unlock_spec
-                            (ret_record.(e_2))
-                            ((st_5.[share].[globals].[g_granules] :<
-                              ((((st_5.(share)).(globals)).(g_granules)) #
-                                ((((test_PA v_1).(meta_granule_offset)) + (4)) / (16)) ==
-                                (((((st_5.(share)).(globals)).(g_granules)) @ ((((test_PA v_1).(meta_granule_offset)) + (4)) / (16))).[e_state_s_granule] :< 5))).[share].[granule_data] :<
-                              (((st_5.(share)).(granule_data)) #
-                                ((((ret_record.(e_2)).(poffset)) + ((8 * ((ret_record.(e_3)))))) / (4096)) ==
-                                ((((st_5.(share)).(granule_data)) @ ((((ret_record.(e_2)).(poffset)) + ((8 * ((ret_record.(e_3)))))) / (4096))).[g_norm] :<
-                                  (((((st_5.(share)).(granule_data)) @ ((((ret_record.(e_2)).(poffset)) + ((8 * ((ret_record.(e_3)))))) / (4096))).(g_norm)) #
-                                    ((((ret_record.(e_2)).(poffset)) + ((8 * ((ret_record.(e_3)))))) mod (4096)) ==
-                                    (test_PTE_Z (mkabs_PTE_t (test_PA v_1) 3 0))))))));
-                      when st_16 == ((granule_unlock_spec (mkPtr "granules" ((test_PA v_1).(meta_granule_offset))) st_15));
-                      (Some (0, st_16)))))
-              | None => None
-              end)
+                    when st_5 == (
+                        (granule_unlock_spec
+                          (mkPtr "granules" (((abs_tte_read (mkPtr "granule_data" (((ret_rtt.(e_2)).(poffset)) + ((8 * ((ret_rtt.(e_3))))))) st_4).(meta_PA)).(meta_granule_offset)))
+                          (st_1.[share].[globals].[g_granules] :<
+                            ((((st_1.(share)).(globals)).(g_granules)) #
+                              ((((abs_tte_read (mkPtr "granule_data" (((ret_rtt.(e_2)).(poffset)) + ((8 * ((ret_rtt.(e_3))))))) st_4).(meta_PA)).(meta_granule_offset)) / (16)) ==
+                              (((((st_1.(share)).(globals)).(g_granules)) @ ((((abs_tte_read (mkPtr "granule_data" (((ret_rtt.(e_2)).(poffset)) + ((8 * ((ret_rtt.(e_3))))))) st_4).(meta_PA)).(meta_granule_offset)) / (16))).[e_ref] :<
+                                ((((((st_1.(share)).(globals)).(g_granules)) @ ((((abs_tte_read (mkPtr "granule_data" (((ret_rtt.(e_2)).(poffset)) + ((8 * ((ret_rtt.(e_3))))))) st_4).(meta_PA)).(meta_granule_offset)) / (16))).(e_ref)).[e_u_anon_3_0] :<
+                                  (g_mapped_addr_set_para
+                                    (((((((st_1.(share)).(globals)).(g_granules)) @ ((((abs_tte_read (mkPtr "granule_data" (((ret_rtt.(e_2)).(poffset)) + ((8 * ((ret_rtt.(e_3))))))) st_4).(meta_PA)).(meta_granule_offset)) / (16))).(e_ref)).(e_u_anon_3_0)) +
+                                      ((- 1)))
+                                    0)))))));
+                    rely ((true = (true)));
+                    rely ((((((ret_rtt.(e_2)).(pbase)) = ("granules")) /\ (((((ret_rtt.(e_2)).(poffset)) mod (16)) = (0)))) /\ ((((ret_rtt.(e_2)).(poffset)) >= (0)))));
+                    when st_20 == (
+                        (granule_unlock_spec
+                          (ret_rtt.(e_2))
+                          ((st_5.[share].[globals].[g_granules] :<
+                            ((((st_5.(share)).(globals)).(g_granules)) #
+                              (((ret_rtt.(e_2)).(poffset)) / (16)) ==
+                              (((((st_5.(share)).(globals)).(g_granules)) @ (((ret_rtt.(e_2)).(poffset)) / (16))).[e_ref] :<
+                                ((((((st_5.(share)).(globals)).(g_granules)) @ (((ret_rtt.(e_2)).(poffset)) / (16))).(e_ref)).[e_u_anon_3_0] :<
+                                  (((((((st_5.(share)).(globals)).(g_granules)) @ (((ret_rtt.(e_2)).(poffset)) / (16))).(e_ref)).(e_u_anon_3_0)) + ((- 1))))))).[share].[granule_data] :<
+                            (((st_5.(share)).(granule_data)) #
+                              ((((ret_rtt.(e_2)).(poffset)) + ((8 * ((ret_rtt.(e_3)))))) / (4096)) ==
+                              ((((st_5.(share)).(granule_data)) @ ((((ret_rtt.(e_2)).(poffset)) + ((8 * ((ret_rtt.(e_3)))))) / (4096))).[g_norm] :<
+                                (((((st_5.(share)).(granule_data)) @ ((((ret_rtt.(e_2)).(poffset)) + ((8 * ((ret_rtt.(e_3)))))) / (4096))).(g_norm)) #
+                                  ((((ret_rtt.(e_2)).(poffset)) + ((8 * ((ret_rtt.(e_3)))))) mod (4096)) ==
+                                  (test_PTE_Z (mkabs_PTE_t (mkabs_PA_t (- 1)) 0 1))))))));
+                    (Some (0, st_20))))
+                else (
+                  when st_2 == (
+                      (spinlock_release_spec
+                        (mkPtr "granules" (((abs_tte_read (mkPtr "granule_data" (((ret_rtt.(e_2)).(poffset)) + ((8 * ((ret_rtt.(e_3))))))) st_4).(meta_PA)).(meta_granule_offset)))
+                        st_1));
+                  if ((pack_struct_return_code_para (make_return_code_para 1)) =? (0))
+                  then (
+                    rely ((((((ret_rtt.(e_2)).(pbase)) = ("granules")) /\ (((((ret_rtt.(e_2)).(poffset)) mod (16)) = (0)))) /\ ((((ret_rtt.(e_2)).(poffset)) >= (0)))));
+                    when st_20 == (
+                        (granule_unlock_spec
+                          (ret_rtt.(e_2))
+                          ((st_2.[share].[globals].[g_granules] :<
+                            ((((st_2.(share)).(globals)).(g_granules)) #
+                              (((ret_rtt.(e_2)).(poffset)) / (16)) ==
+                              (((((st_2.(share)).(globals)).(g_granules)) @ (((ret_rtt.(e_2)).(poffset)) / (16))).[e_ref] :<
+                                ((((((st_2.(share)).(globals)).(g_granules)) @ (((ret_rtt.(e_2)).(poffset)) / (16))).(e_ref)).[e_u_anon_3_0] :<
+                                  (((((((st_2.(share)).(globals)).(g_granules)) @ (((ret_rtt.(e_2)).(poffset)) / (16))).(e_ref)).(e_u_anon_3_0)) + ((- 1))))))).[share].[granule_data] :<
+                            (((st_2.(share)).(granule_data)) #
+                              ((((ret_rtt.(e_2)).(poffset)) + ((8 * ((ret_rtt.(e_3)))))) / (4096)) ==
+                              ((((st_2.(share)).(granule_data)) @ ((((ret_rtt.(e_2)).(poffset)) + ((8 * ((ret_rtt.(e_3)))))) / (4096))).[g_norm] :<
+                                (((((st_2.(share)).(granule_data)) @ ((((ret_rtt.(e_2)).(poffset)) + ((8 * ((ret_rtt.(e_3)))))) / (4096))).(g_norm)) #
+                                  ((((ret_rtt.(e_2)).(poffset)) + ((8 * ((ret_rtt.(e_3)))))) mod (4096)) ==
+                                  (test_PTE_Z (mkabs_PTE_t (mkabs_PA_t (- 1)) 0 1))))))));
+                    (Some (0, st_20)))
+                  else (
+                    when st_14 == ((granule_unlock_spec (ret_rtt.(e_2)) st_2));
+                    (Some ((pack_struct_return_code_para (make_return_code_para 1)), st_14))))))
             else (
-              when st_7 == ((granule_unlock_spec (ret_record.(e_2)) st_4));
-              when st_8 == ((granule_unlock_spec (mkPtr "granules" ((test_PA v_1).(meta_granule_offset))) st_7));
-              (Some ((pack_struct_return_code_para (make_return_code_para 8)), st_8)))))
-        else (Some ((pack_struct_return_code_para (make_return_code_para 1)), st')));
-    ((Some v_7), st_2).
+              when st_13 == ((granule_unlock_spec (ret_rtt.(e_2)) st_4));
+              (Some ((pack_struct_return_code_para (make_return_code_para 9)), st_13)))))
+        else (
+          when st_12 == ((granule_unlock_spec (ret_rtt.(e_2)) st_4));
+          (Some (0, st_12)))))
+    else (
+      when st_8 == ((granule_unlock_spec (ret_rtt.(e_2)) st_4));
+      (Some ((pack_struct_return_code_para (make_return_code_para 8)), st_8))).
 
 End Layer8_Spec.
 
 #[global] Hint Unfold rtt_create_s1_el1_spec_abs: spec.
-#[global] Hint Unfold rtt_create_s1_el1_spec: spec.
+#[global] Hint Unfold map_unmap_ns_s1_0: spec.
+#[global] Hint Unfold map_unmap_ns_s1_1: spec.
+#[global] Hint Unfold map_unmap_ns_s1_2: spec.
+#[global] Hint Unfold map_unmap_ns_s1_3: spec.
+#[global] Hint Unfold map_unmap_ns_s1_spec: spec.
