container/coq/pointer/Layer8/map_unmap_ns_s1/LowSpec.v
@@ -1,0 +1,139 @@
+Require Import Code.
+Require Import CommonDeps.
+Require Import DataTypes.
+Require Import GlobalDefs.
+
+Local Open Scope string_scope.
+Local Open Scope Z_scope.
+
+Section Layer8_map_unmap_ns_s1_LowSpec.
+
+  Context `{int_ptr: IntPtrCast}.
+
+  Definition map_unmap_ns_s1_0_low (st_0: RData) (st_12: RData) (v_17: Ptr) (v_3: abs_PTE_t) (v_31: Z) (v__sroa_0_0_copyload: Ptr) (v__sroa_7_0_copyload: Z) : (option (Z * RData)) :=
+    rely (((v_31 =? (0)) = (true)));
+    when st_14 == ((stage1_tlbi_all_spec st_12));
+    when st_15 == ((__tte_write_spec_abs (ptr_offset v_17 (8 * (v__sroa_7_0_copyload))) v_3 st_14));
+    when st_16 == ((iasm_8_spec st_15));
+    when st_17 == ((iasm_12_isb_spec st_16));
+    when st_18 == ((__granule_get_spec v__sroa_0_0_copyload st_17));
+    when st_19 == ((granule_unlock_spec v__sroa_0_0_copyload st_18));
+    when st_20 == ((free_stack "map_unmap_ns_s1" st_0 st_19));
+    (Some (0, st_20)).
+
+  Definition map_unmap_ns_s1_1_low (st_0: RData) (st_11: RData) (v_17: Ptr) (v_3: abs_PTE_t) (v__sroa_0_0_copyload: Ptr) (v__sroa_7_0_copyload: Z) : (option (Z * RData)) :=
+    when st_13 == ((stage1_tlbi_all_spec st_11));
+    when st_14 == ((__tte_write_spec_abs (ptr_offset v_17 (8 * (v__sroa_7_0_copyload))) v_3 st_13));
+    when st_15 == ((iasm_8_spec st_14));
+    when st_16 == ((iasm_12_isb_spec st_15));
+    when st_17 == ((__granule_get_spec v__sroa_0_0_copyload st_16));
+    when st_18 == ((granule_unlock_spec v__sroa_0_0_copyload st_17));
+    when st_19 == ((free_stack "map_unmap_ns_s1" st_0 st_18));
+    (Some (0, st_19)).
+
+  Definition map_unmap_ns_s1_2_low (st_0: RData) (st_12: RData) (v_17: Ptr) (v_47: Z) (v__sroa_0_0_copyload: Ptr) (v__sroa_7_0_copyload: Z) : (option (Z * RData)) :=
+    rely (((v_47 =? (0)) = (true)));
+    when v_51, st_14 == ((s2tte_create_unassigned_spec_abs 1 st_12));
+    when st_15 == ((__tte_write_spec_abs (ptr_offset v_17 (8 * (v__sroa_7_0_copyload))) v_51 st_14));
+    when st_16 == ((iasm_8_spec st_15));
+    when st_17 == ((iasm_12_isb_spec st_16));
+    when st_18 == ((stage1_tlbi_all_spec st_17));
+    when st_19 == ((__granule_put_spec v__sroa_0_0_copyload st_18));
+    when st_20 == ((granule_unlock_spec v__sroa_0_0_copyload st_19));
+    when st_21 == ((free_stack "map_unmap_ns_s1" st_0 st_20));
+    (Some (0, st_21)).
+
+  Definition map_unmap_ns_s1_3_low (st_0: RData) (st_11: RData) (v_17: Ptr) (v_20: abs_PTE_t) (v__sroa_0_0_copyload: Ptr) (v__sroa_7_0_copyload: Z) : (option (Z * RData)) :=
+    when v_51, st_13 == ((s2tte_create_unassigned_spec_abs 1 st_11));
+    when st_14 == ((__tte_write_spec_abs (ptr_offset v_17 (8 * (v__sroa_7_0_copyload))) v_51 st_13));
+    when st_15 == ((iasm_8_spec st_14));
+    when st_16 == ((iasm_12_isb_spec st_15));
+    when st_17 == ((stage1_tlbi_all_spec st_16));
+    when st_18 == ((__granule_put_spec v__sroa_0_0_copyload st_17));
+    when st_19 == ((granule_unlock_spec v__sroa_0_0_copyload st_18));
+    when st_20 == ((free_stack "map_unmap_ns_s1" st_0 st_19));
+    (Some (0, st_20)).
+
+  Definition map_unmap_ns_s1_spec_low (v_0_Zptr: Z) (v_1: Z) (v_2: Z) (v_3: Z) (v_4: Z) (st: RData) : (option (Z * RData)) :=
+    let v_3_pte := (test_Z_PTE v_3) in
+    when st_0 == ((new_frame "map_unmap_ns_s1" st));
+    when v_8, st_1 == ((find_granule_spec_abs (test_PA v_0_Zptr) st_0));
+    rely ((((v_8.(pbase)) = ("granules")) \/ (((v_8.(pbase)) = ("null")))));
+    if (ptr_eqb v_8 (mkPtr "null" 0))
+    then (
+      when v_10, st_2 == ((pack_return_code_spec 1 1 st_1));
+      when st_4 == ((free_stack "map_unmap_ns_s1" st_0 st_2));
+      (Some (v_10, st_4)))
+    else (
+      when st_3 == ((granule_lock_spec v_8 5 st_1));
+      when ret_rtt, st_4 == ((rtt_walk_lock_unlock_spec_abs (mkPtr "stack_s_rtt_walk" 0) v_8 0 64 v_1 v_2 st_3));
+      rely ((((st_4.(share)).(granule_data)) = (((st_3.(share)).(granule_data)))));
+      let v__sroa_0_0_copyload := (ret_rtt.(e_2)) in
+      let v__sroa_10_0_copyload := (ret_rtt.(e_1)) in
+      let st_6 := st_4 in
+      if ((v__sroa_10_0_copyload - (v_2)) =? (0))
+      then (
+        let st_8 := st_6 in
+        let v__sroa_7_0_copyload := (ret_rtt.(e_3)) in
+        when v_17, st_9 == ((granule_map_spec v__sroa_0_0_copyload 6 st_8));
+        when v_20, st_10 == ((abs__tte_read_spec (ptr_offset v_17 (8 * (v__sroa_7_0_copyload))) st_9));
+        if (v_4 =? (0))
+        then (
+          when v_23, st_11 == ((s2tte_is_unassigned_spec_abs v_20 st_10));
+          if v_23
+          then (
+            if (uart0_phys_para v_3_pte)
+            then (map_unmap_ns_s1_1_low st_0 st_11 v_17 v_3_pte v__sroa_0_0_copyload v__sroa_7_0_copyload)
+            else (
+              when v_31, st_12 == ((smc_granule_ns_to_any_spec_abs v_1 (v_3_pte.(meta_PA)) st_11));
+              if (v_31 =? (0))
+              then (map_unmap_ns_s1_0_low st_0 st_12 v_17 v_3_pte v_31 v__sroa_0_0_copyload v__sroa_7_0_copyload)
+              else (
+                when v_33, st_13 == ((pack_return_code_spec 1 4 st_12));
+                when st_14 == ((granule_unlock_spec v__sroa_0_0_copyload st_13));
+                when st_16 == ((free_stack "map_unmap_ns_s1" st_0 st_14));
+                (Some (v_33, st_16)))))
+          else (
+            when v_25, st_12 == ((pack_return_code_spec 9 0 st_11));
+            when st_13 == ((granule_unlock_spec v__sroa_0_0_copyload st_12));
+            when st_15 == ((free_stack "map_unmap_ns_s1" st_0 st_13));
+            (Some (v_25, st_15))))
+        else (
+          if (v_4 =? (1))
+          then (
+            when v_39, st_11 == ((s1tte_is_valid_spec_abs v_20 v_2 st_10));
+            if v_39
+            then (
+              if (uart0_phys_para v_20)
+              then (map_unmap_ns_s1_3_low st_0 st_11 v_17 v_20 v__sroa_0_0_copyload v__sroa_7_0_copyload)
+              else (
+                when v_47, st_12 == ((smc_granule_any_to_ns_spec_abs (v_20.(meta_PA)) st_11));
+                if (v_47 =? (0))
+                then (map_unmap_ns_s1_2_low st_0 st_12 v_17 v_47 v__sroa_0_0_copyload v__sroa_7_0_copyload)
+                else (
+                  when v_49, st_13 == ((pack_return_code_spec 1 2 st_12));
+                  when st_14 == ((granule_unlock_spec v__sroa_0_0_copyload st_13));
+                  when st_16 == ((free_stack "map_unmap_ns_s1" st_0 st_14));
+                  (Some (v_49, st_16)))))
+            else (
+              when v_41, st_12 == ((pack_return_code_spec 9 0 st_11));
+              when st_13 == ((granule_unlock_spec v__sroa_0_0_copyload st_12));
+              when st_15 == ((free_stack "map_unmap_ns_s1" st_0 st_13));
+              (Some (v_41, st_15))))
+          else (
+            when st_12 == ((granule_unlock_spec v__sroa_0_0_copyload st_10));
+            when st_13 == ((free_stack "map_unmap_ns_s1" st_0 st_12));
+            (Some (0, st_13)))))
+      else (
+        when v_15, st_7 == ((pack_return_code_spec 8 v__sroa_10_0_copyload st_6));
+        when st_8 == ((granule_unlock_spec v__sroa_0_0_copyload st_7));
+        when st_10 == ((free_stack "map_unmap_ns_s1" st_0 st_8));
+        (Some (v_15, st_10)))).
+
+End Layer8_map_unmap_ns_s1_LowSpec.
+
+#[global] Hint Unfold map_unmap_ns_s1_0_low: spec.
+#[global] Hint Unfold map_unmap_ns_s1_1_low: spec.
+#[global] Hint Unfold map_unmap_ns_s1_2_low: spec.
+#[global] Hint Unfold map_unmap_ns_s1_3_low: spec.
+#[global] Hint Unfold map_unmap_ns_s1_spec_low: spec.
